clightplus/compiler_proof/ClightPlus2ClightLenv.v
@@ -4,14 +4,11 @@ Require Import CoqlibCCR.
 Require Import PCM.
 Require Import AList.
 
-Require Import ClightPlus2ClightMatch.
+Require Import ClightPlus2ClightMatchEnv.
 
 Set Implicit Arguments.
 
 Section LENV.
-
-  Context `{Σ: GRA.t}.
-  Context `{builtins : builtinsTy}.
 
   (* Lemma match_update_le sk defs le tle o v
         (MLE: match_le sk defs le tle)
@@ -22,6 +19,63 @@ Section LENV.
     - subst. rewrite PTree.gss in *. clarify.
     - rewrite PTree.gso in *; et.
   Qed. *)
+
+
+  Lemma match_sizeof ty ce tce
+      (MCE: match_ce ce tce)
+    :
+      Ctypes.sizeof tce ty = ClightPlusExprgen.sizeof ce ty.
+  Proof.
+    induction ty; ss.
+    - rewrite IHty. et.
+    - destruct (tce ! i) eqn:?; destruct alist_find eqn:?.
+      + eapply cenv_match_some in Heqo0; et. clarify.
+      + eapply cenv_match_none in Heqo0; et. clarify.
+      + eapply cenv_match_some in Heqo0; et. clarify.
+      + et.
+    - destruct (tce ! i) eqn:?; destruct alist_find eqn:?.
+      + eapply cenv_match_some in Heqo0; et. clarify.
+      + eapply cenv_match_none in Heqo0; et. clarify.
+      + eapply cenv_match_some in Heqo0; et. clarify.
+      + et.
+  Qed.
+
+  Lemma match_alignof_blockcopy ty ce tce
+      (MCE: match_ce ce tce)
+    :
+      Ctypes.alignof_blockcopy tce ty = ClightPlusExprgen.alignof_blockcopy ce ty.
+  Proof.
+    induction ty; ss.
+    - destruct (tce ! i) eqn:?; destruct alist_find eqn:?.
+      + eapply cenv_match_some in Heqo0; et. clarify.
+      + eapply cenv_match_none in Heqo0; et. clarify.
+      + eapply cenv_match_some in Heqo0; et. clarify.
+      + et.
+    - destruct (tce ! i) eqn:?; destruct alist_find eqn:?.
+      + eapply cenv_match_some in Heqo0; et. clarify.
+      + eapply cenv_match_none in Heqo0; et. clarify.
+      + eapply cenv_match_some in Heqo0; et. clarify.
+      + et.
+  Qed.
+
+  Lemma match_alignof ty ce tce
+      (MCE: match_ce ce tce)
+    :
+      Ctypes.alignof tce ty = ClightPlusExprgen.alignof ce ty.
+  Proof.
+    induction ty; ss.
+    - rewrite IHty. et.
+    - destruct (tce ! i) eqn:?; destruct alist_find eqn:?.
+      + eapply cenv_match_some in Heqo0; et. clarify.
+      + eapply cenv_match_none in Heqo0; et. clarify.
+      + eapply cenv_match_some in Heqo0; et. clarify.
+      + et.
+    - destruct (tce ! i) eqn:?; destruct alist_find eqn:?.
+      + eapply cenv_match_some in Heqo0; et. clarify.
+      + eapply cenv_match_none in Heqo0; et. clarify.
+      + eapply cenv_match_some in Heqo0; et. clarify.
+      + et.
+  Qed.
 
   Lemma update_le
         sk defs x id v sv le tle
