clightplus/compiler_proof/ClightPlus2ClightSim.v
@@ -11,14 +11,14 @@ Require Import STS2SmallStep.
 Require Import ClightPlusMem0.
 Require Import IRed.
 
-Require Import ClightPlus2ClightMatch.
+Require Import ClightPlus2ClightMatchEnv.
 Require Import ClightPlus2ClightArith.
 Require Import ClightPlus2ClightLenv.
 Require Import ClightPlus2ClightMem.
 
 From compcert Require Import Ctypes Clight Clightdefs Values.
 
-(* Lemma unbind_trigger E:
+Lemma unbind_trigger E:
   forall [X0 X1 A : Type] (ktr0 : X0 -> itree E A) (ktr1 : X1 -> itree E A) e0 e1,
     (x <- trigger e0;; ktr0 x = x <- trigger e1;; ktr1 x) -> (X0 = X1 /\ e0 ~= e1 /\ ktr0 ~= ktr1).
 Proof.
@@ -28,30 +28,29 @@ Proof.
   cbv in x. subst. split; auto.
   assert (ktr0 = ktr1); clarify.
   extensionality x. eapply equal_f in x0.
-  rewrite ! subst_bind in *.
   irw in x0. eauto.
-Qed. *)
+Qed.
 
-(* Lemma angelic_step :
+Lemma angelic_step :
   forall (X : Prop) (ktr next : itree eventE Any.t),
     ModSemL.step (trigger (Take X);;; ktr) None next -> (next = ktr /\ X).
 Proof.
   i. dependent destruction H; try (irw in x; clarify; fail).
   rewrite <- bind_trigger in x. apply unbind_trigger in x.
   des. clarify.
-Qed. *)
+Qed.
 
-(* Lemma eval_exprlist_length :
-  forall a b c d l1 l2
-    (EE: eval_exprlist a b c d l1 l2),
+Lemma eval_exprlist_length :
+  forall a b c d l1 tl l2
+    (EE: eval_exprlist a b c d l1 tl l2),
     <<EELEN: List.length l1 = List.length l2>>.
 Proof.
   i. induction EE; ss; clarify; eauto.
-Qed. *)
+Qed.
 
 Section PROOF.
 
-  (* Import ModSemL.
+  Import ModSemL.
 
   Context `{Σ: GRA.t}.
   Context `{builtins : builtinsTy}.
@@ -104,7 +103,9 @@ Section PROOF.
 
   Ltac wrap_up := try pfold; econs 7; et; right.
 
-  Ltac remove_UBcase := des_ifs; try sim_red; try sim_triggerUB.
+  Ltac remove_UBcase := des_ifs; try sim_red; try solve [sim_triggerUB].
+
+  Ltac step := repeat (sim_red; try sim_tau).
 
   Ltac eapplyf NEXT := let X := fresh "X" in hexploit NEXT;[..|intro X; punfold X; et].
   Ltac dtm H H0 := eapply angelic_step in H; eapply angelic_step in H0; des; rewrite H; rewrite H0; ss.
@@ -141,10 +142,13 @@ Section PROOF.
     unfold ccallU. sim_red. 
     sim_tau. ss. sim_red. unfold loadF. repeat (sim_red; sim_tau). sim_red.
     rewrite PSTATE. sim_red. unfold unwrapU. remove_UBcase. sim_tau. sim_red. rewrite Any.upcast_downcast.
-    sim_red. eapplyf NEXT. unfold Mem.loadv in *. des_ifs_safe. ss. clarify. hexploit match_mem_load; et.
+    sim_red. eapplyf NEXT. unfold Mem.loadv in *. des_ifs_safe.
+    destruct addr; ss; cycle 1.
+    - hexploit match_mem_load; et.
+    - destruct Mem.denormalize eqn:? in Heq; clarify.
+      destruct p. hexploit match_mem_denormalize; et.
+      i. rewrite H. hexploit match_mem_load; et.
   Qed.
-  
-    
 
   Lemma step_store pstate f_table modl cprog sk tge le tle e te m tm
     (PSTATE: pstate "Mem"%string = m↑)
@@ -174,10 +178,66 @@ Section PROOF.
   Proof.
     unfold ccallU. sim_red. sim_tau. ss. sim_red. unfold storeF. sim_red. repeat (sim_tau; sim_red).
     rewrite PSTATE. sim_red. unfold unwrapU. remove_UBcase. repeat (sim_tau; sim_red). rewrite Any.upcast_downcast.
-    sim_red. unfold Mem.storev in Heq. des_ifs_safe. hexploit match_mem_store; et. i. des. eapplyf NEXT; et. 
+    sim_red. unfold Mem.storev in Heq. des_ifs.
+    - hexploit match_mem_denormalize; et. i. 
+      hexploit match_mem_store; et. i. des. eapplyf NEXT; et.
+      unfold Mem.storev. ss. des_ifs.
+    - hexploit match_mem_store; et. i. des. eapplyf NEXT; et.
   Qed.
 
-  Lemma step_loadbytes pstate f_table modl cprog sk tge le tle e te m tm
+  Lemma step_memcpy pstate f_table modl cprog sk tge le tle e te m tm
+    (PSTATE: pstate "Mem"%string = m↑)
+    (EQ: f_table = (ModL.add Mem modl).(ModL.enclose))
+    (MGE: match_ge sk tge)
+    (ME: match_e sk tge e te)
+    (MLE: match_le sk tge le tle)
+    (MM: match_mem sk tge m tm)
+    al sz vp v
+    tf tcode tcont ktr b r mn
+    (NEXT: forall tm' m',
+            extcall_memcpy_sem sz al tge [map_val sk tge vp; map_val sk tge v] tm E0 Vundef tm' ->
+            match_mem sk tge m' tm' ->
+            paco4
+              (_sim (ModL.compile (ModL.add Mem modl)) (semantics2 cprog)) r true b
+              (ktr (update pstate "Mem" m'↑, Vundef))
+              (State tf tcode tcont te tle tm))
+:
+    paco4
+      (_sim (ModL.compile (ModL.add Mem modl)) (semantics2 cprog)) r true b
+      (`r0: p_state * val <- 
+        (EventsL.interp_Es
+          (prog f_table)
+          (transl_all mn (ccallU "memcpy" (al, sz, [vp; v]))) 
+          pstate);; ktr r0)
+      (State tf tcode tcont te tle tm).
+  Proof.
+    unfold ccallU. sim_red. sim_tau. ss. sim_red. destruct dec.
+    - sim_red. sim_tau. sim_red. hexploit NEXT; et. { econs 2. et. }
+      i. punfold H. assert (update pstate "Mem" m↑ = pstate).
+      { extensionalities. unfold update. destruct dec; et. subst. et. }
+      rewrite H0 in H. et.
+    - repeat (sim_red; sim_tau). sim_red. rewrite PSTATE.
+      rewrite Any.upcast_downcast. sim_red.
+      unfold unwrapU. remove_UBcase. remove_UBcase. remove_UBcase.
+      repeat ((repeat sim_red); sim_tau). sim_red.
+      rewrite Any.upcast_downcast. sim_red.
+      hexploit match_to_ptr; et. i. move Heq at bottom.
+      hexploit match_to_ptr; et. i. ss.
+      hexploit match_mem_loadbytes; et. i.
+      hexploit match_mem_storebytes; et. i. des.
+      eapplyf NEXT; et.
+      bsimpl. repeat destruct Zdivide_dec; ss; try nia.
+      repeat destruct Coqlib.zle; ss; try nia.
+      repeat destruct dec; ss; try nia.
+      all: econs; et; try nia.
+      + repeat destruct dec; ss; et; des; clarify.
+      + repeat destruct dec; ss; et; des; clarify.
+      + destruct (dec (Ptrofs.unsigned _) _) in Heq2; et.
+        left. ss. destruct (dec b1 b0); ss; des; clarify.
+        all: ii; apply n1; eapply map_blk_inj; et.
+  Qed.
+
+  (* Lemma step_loadbytes pstate f_table modl cprog sk tge le tle e te m tm
     (PSTATE: pstate "Mem"%string = m↑)
     (EQ: f_table = (ModL.add Mem modl).(ModL.enclose))
     (MGE: match_ge sk tge)
@@ -298,18 +358,225 @@ Section PROOF.
       eapply step_load; et; i; remove_UBcase; 
         eapply step_store; et; i; sim_red;
           eapplyf NEXT; et; econs; et; try nia; des_ifs.
-  Qed.
+  Qed. *)
 
-  Lemma step_weak_valid_pointer pstate f_table modl cprog sk tge le tle e te m tm
+  Lemma step_sub_ptr pstate f_table modl cprog sk tge le tle e te m tm
     (PSTATE: pstate "Mem"%string = m↑)
     (EQ: f_table = (ModL.add Mem modl).(ModL.enclose))
     (ME: match_e sk tge e te)
     (MLE: match_le sk tge le tle)
+    (MGE: match_ge sk tge)
     (MM: match_mem sk tge m tm)
-    blk ofs
+    sz v1 v2
+    tf tcode tcont ktr bflag r mn
+    (NEXT: forall ofs,
+          Cop._sem_ptr_sub_join_common (map_val sk tge v1) (map_val sk tge v2) tm = Some ofs ->
+          (0 < sz <= Ptrofs.max_signed)%Z ->
+            paco4
+              (_sim (ModL.compile (ModL.add Mem modl)) (semantics2 cprog)) r true bflag
+              (ktr (pstate, Vptrofs (Ptrofs.divs ofs (Ptrofs.repr sz))))
+              (State tf tcode tcont te tle tm))
+:
+    paco4
+      (_sim (ModL.compile (ModL.add Mem modl)) (semantics2 cprog)) r true bflag
+      (`r0: (p_state * val) <- 
+        (EventsL.interp_Es
+          (prog f_table)
+          (transl_all mn (ccallU "sub_ptr" (sz, v1, v2))) 
+          pstate);; ktr r0)
+      (State tf tcode tcont te tle tm).
+  Proof.
+    unfold ccallU. sim_red. sim_tau. ss. sim_red. unfold sub_ptrF. sim_tau. repeat (sim_tau; sim_red).
+    rewrite PSTATE. sim_red. unfold unwrapU. remove_UBcase.
+    repeat (sim_tau; sim_red). rewrite Any.upcast_downcast. sim_red.
+    destruct Coqlib.zlt; destruct Coqlib.zle; ss.
+    eapplyf NEXT; et; try nia.
+    unfold Cop._sem_ptr_sub_join_common in *.
+    des_ifs; ss; clarify.
+    - unfold Cop._sem_ptr_sub_join, Cop._sem_ptr_sub in *. des_ifs.
+    - unfold Cop._sem_ptr_sub_join in Heq0. des_ifs.
+      + unfold Cop._sem_ptr_sub in *. des_ifs.
+        unfold IntPtrRel.to_ptr_val, IntPtrRel.option_to_val in *.
+        unfold IntPtrRel.to_int_val, IntPtrRel.option_to_val in *.
+        des_ifs. move Heq6 at bottom.
+        hexploit match_to_ptr; et. i.
+        hexploit match_to_int; et. i.
+        simpl in Heq0. simpl in Heq4. simpl map_val in H. simpl map_val in H0.
+        clarify.
+        unfold Cop._sem_ptr_sub_join.
+        unfold Cop._sem_ptr_sub, IntPtrRel.to_int_val, IntPtrRel.to_ptr_val, IntPtrRel.option_to_val.
+        rewrite H. rewrite H0. des_ifs.
+        { simpl in Heq0. clarify. }
+        { simpl in Heq0. simpl in Heq2. clarify. }
+        { f_equal. symmetry. simpl in Heq2. clarify. apply Ptrofs.same_if_eq. et. }
+      + unfold Cop._sem_ptr_sub in Heq1. des_ifs.
+        unfold IntPtrRel.to_ptr_val, IntPtrRel.option_to_val in *.
+        des_ifs. move Heq3 at bottom.
+        hexploit match_to_ptr; et. i.
+        simpl in Heq1. simpl map_val in H. clarify.
+        unfold Cop._sem_ptr_sub_join.
+        unfold Cop._sem_ptr_sub, IntPtrRel.to_ptr_val, IntPtrRel.option_to_val.
+        rewrite H. des_ifs.
+        all: try solve [ss; clarify].
+        simpl in Heq0. unfold IntPtrRel.to_int_val in Heq5. simpl in Heq5. clarify. 
+        clear - Heq6 H Heq4.
+        unfold IntPtrRel.to_int_val, IntPtrRel.option_to_val in Heq6.
+        des_ifs. unfold Mem.to_ptr, Mem.to_int, Mem.ptr2int_v, Mem.ptr2int in *.
+        des_ifs. unfold Mem.denormalize in *. apply Maps.PTree.gselectf in Heq2.
+        des. unfold Mem.denormalize_aux, Mem.is_valid, Mem.addr_is_in_block in Heq3.
+        des_ifs; bsimpl; clarify. des.
+        clear - Heq4. hexploit Ptrofs.eq_spec. rewrite Heq4. i. exfalso.
+        apply H. unfold Ptrofs.of_int64, Ptrofs.sub, Int64.sub.
+        apply Ptrofs.eqm_samerepr. rewrite <- Ptrofs.eqm64; et.
+        eapply Int64.eqm_trans. 2:{ apply Int64.eqm_unsigned_repr. }
+        eapply Int64.eqm_trans.
+        2:{ apply Int64.eqm_sub. apply Int64.eqm_refl. apply Int64.eqm_unsigned_repr. }
+        eapply Int64.eqm_trans.
+        { apply Int64.eqm_sub. apply Int64.eqm_sym. apply Int64.eqm_unsigned_repr. apply Int64.eqm_refl. }
+        eapply Int64.eqm_refl2. nia.
+      + unfold Cop._sem_ptr_sub in Heq2. des_ifs.
+        unfold IntPtrRel.to_int_val, IntPtrRel.option_to_val in *.
+        des_ifs. hexploit match_to_int; et. i.
+        simpl in Heq3. simpl map_val in H. clarify.
+        unfold Cop._sem_ptr_sub_join.
+        unfold Cop._sem_ptr_sub, IntPtrRel.to_int_val, IntPtrRel.option_to_val.
+        rewrite H. des_ifs.
+        { ss. clarify. f_equal. apply Ptrofs.same_if_eq. et. }
+        unfold IntPtrRel.to_ptr_val in Heq7. simpl in Heq7, Heq3. clarify.
+        clear - Heq6 H Heq5.
+        unfold IntPtrRel.to_ptr_val, IntPtrRel.option_to_val in Heq6.
+        des_ifs. unfold Mem.to_ptr, Mem.to_int, Mem.ptr2int_v, Mem.ptr2int in *.
+        des_ifs. unfold Mem.denormalize in *. apply Maps.PTree.gselectf in Heq2.
+        des. unfold Mem.denormalize_aux, Mem.is_valid, Mem.addr_is_in_block in Heq4.
+        des_ifs; bsimpl; clarify. des.
+        clear - Heq5. hexploit Ptrofs.eq_spec. rewrite Heq5. i. exfalso.
+        apply H. unfold Ptrofs.of_int64, Ptrofs.sub, Int64.sub.
+        apply Ptrofs.eqm_samerepr. rewrite <- Ptrofs.eqm64; et.
+        eapply Int64.eqm_trans. 2:{ apply Int64.eqm_unsigned_repr. }
+        eapply Int64.eqm_trans.
+        2:{ apply Int64.eqm_sub. apply Int64.eqm_refl. apply Int64.eqm_unsigned_repr. }
+        eapply Int64.eqm_trans.
+        { apply Int64.eqm_sub. apply Int64.eqm_sym. apply Int64.eqm_unsigned_repr. apply Int64.eqm_refl. }
+        eapply Int64.eqm_refl2. nia.
+    - unfold Cop._sem_ptr_sub_join, Cop._sem_ptr_sub in *. des_ifs.
+    - unfold Cop._sem_ptr_sub_join in Heq0. des_ifs.
+      + unfold Cop._sem_ptr_sub in *. des_ifs.
+        unfold IntPtrRel.to_ptr_val, IntPtrRel.option_to_val in *.
+        unfold IntPtrRel.to_int_val, IntPtrRel.option_to_val in *.
+        des_ifs. hexploit match_to_ptr; et. i.
+        move Heq4 at bottom.
+        hexploit match_to_int; et. i.
+        simpl in Heq6. simpl in Heq1. simpl map_val in H. simpl map_val in H0.
+        clarify.
+        unfold Cop._sem_ptr_sub_join.
+        unfold Cop._sem_ptr_sub, IntPtrRel.to_int_val, IntPtrRel.to_ptr_val, IntPtrRel.option_to_val.
+        rewrite H. rewrite H0. des_ifs.
+        { simpl in Heq1. clarify. }
+        { simpl in Heq1. simpl in Heq2. clarify. }
+        { f_equal. symmetry. simpl in Heq2. clarify. apply Ptrofs.same_if_eq. et. }
+      + unfold Cop._sem_ptr_sub in Heq1. des_ifs.
+        unfold IntPtrRel.to_ptr_val, IntPtrRel.option_to_val in *.
+        des_ifs.
+        hexploit match_to_ptr; et. i.
+        simpl in Heq3. simpl map_val in H. clarify.
+        unfold Cop._sem_ptr_sub_join.
+        unfold Cop._sem_ptr_sub, IntPtrRel.to_ptr_val, IntPtrRel.option_to_val.
+        rewrite H. des_ifs.
+        all: try solve [ss; clarify].
+        simpl in Heq0. unfold IntPtrRel.to_int_val in Heq6. simpl in Heq6. clarify.
+        clear - Heq5 H Heq4.
+        unfold IntPtrRel.to_int_val, IntPtrRel.option_to_val in Heq5.
+        des_ifs. unfold Mem.to_ptr, Mem.to_int, Mem.ptr2int_v, Mem.ptr2int in *.
+        des_ifs. unfold Mem.denormalize in *. apply Maps.PTree.gselectf in Heq2.
+        des. unfold Mem.denormalize_aux, Mem.is_valid, Mem.addr_is_in_block in Heq3.
+        des_ifs; bsimpl; clarify. des.
+        clear - Heq4. hexploit Ptrofs.eq_spec. rewrite Heq4. i. exfalso.
+        apply H. unfold Ptrofs.of_int64, Ptrofs.sub, Int64.sub.
+        apply Ptrofs.eqm_samerepr. rewrite <- Ptrofs.eqm64; et.
+        eapply Int64.eqm_trans. 2:{ apply Int64.eqm_unsigned_repr. }
+        eapply Int64.eqm_trans.
+        2:{ apply Int64.eqm_sub. apply Int64.eqm_unsigned_repr. apply Int64.eqm_refl. }
+        eapply Int64.eqm_trans.
+        { apply Int64.eqm_sub. apply Int64.eqm_refl. apply Int64.eqm_sym. apply Int64.eqm_unsigned_repr. }
+        eapply Int64.eqm_refl2. nia.
+      + unfold Cop._sem_ptr_sub in Heq2. des_ifs.
+        unfold IntPtrRel.to_int_val, IntPtrRel.option_to_val in *.
+        des_ifs. move Heq3 at bottom.
+        hexploit match_to_int; et. i.
+        simpl in Heq2. simpl map_val in H. clarify.
+        unfold Cop._sem_ptr_sub_join.
+        unfold Cop._sem_ptr_sub, IntPtrRel.to_int_val, IntPtrRel.option_to_val.
+        rewrite H. des_ifs.
+        { ss. clarify. f_equal. apply Ptrofs.same_if_eq. et. }
+        unfold IntPtrRel.to_ptr_val in Heq6. simpl in Heq6, Heq2. clarify.
+        clear - Heq7 H Heq5.
+        unfold IntPtrRel.to_ptr_val, IntPtrRel.option_to_val in Heq7.
+        des_ifs. unfold Mem.to_ptr, Mem.to_int, Mem.ptr2int_v, Mem.ptr2int in *.
+        des_ifs. unfold Mem.denormalize in *. apply Maps.PTree.gselectf in Heq2.
+        des. unfold Mem.denormalize_aux, Mem.is_valid, Mem.addr_is_in_block in Heq4.
+        des_ifs; bsimpl; clarify. des.
+        clear - Heq5. hexploit Ptrofs.eq_spec. rewrite Heq5. i. exfalso.
+        apply H. unfold Ptrofs.of_int64, Ptrofs.sub, Int64.sub.
+        apply Ptrofs.eqm_samerepr. rewrite <- Ptrofs.eqm64; et.
+        eapply Int64.eqm_trans. 2:{ apply Int64.eqm_unsigned_repr. }
+        eapply Int64.eqm_trans.
+        2:{ apply Int64.eqm_sub. apply Int64.eqm_unsigned_repr. apply Int64.eqm_refl. }
+        eapply Int64.eqm_trans.
+        { apply Int64.eqm_sub. apply Int64.eqm_refl. apply Int64.eqm_sym. apply Int64.eqm_unsigned_repr. }
+        eapply Int64.eqm_refl2. nia.
+    - destruct eq_block eqn:? in Heq0; clarify. 
+      subst. destruct eq_block; clarify.
+  Qed.
+
+  Lemma match_to_ptr_val m tm sk tge v b ofs
+    (MM: match_mem sk tge m tm)
+    (MGE: match_ge sk tge)
+    (SVAL: IntPtrRel.to_ptr_val m v = Vptr b ofs)
+  : 
+    IntPtrRel.to_ptr_val tm (map_val sk tge v) = Vptr (map_blk sk tge b) ofs.
+  Proof.
+    unfold IntPtrRel.to_ptr_val in *. destruct (Mem.to_ptr _ tm) eqn:?; destruct (Mem.to_ptr _ m) eqn:?; ss; clarify.
+    - hexploit match_to_ptr; et. i. clarify.
+    - hexploit match_to_ptr; et. i. clarify.
+  Qed.
+
+  Lemma match_to_int_val m tm sk tge v i
+    (MM: match_mem sk tge m tm)
+    (MGE: match_ge sk tge)
+    (SVAL: IntPtrRel.to_int_val m v = Vlong i)
+  : 
+    IntPtrRel.to_int_val tm (map_val sk tge v) = Vlong i.
+  Proof.
+    unfold IntPtrRel.to_int_val in *. destruct (Mem.to_int _ tm) eqn:?; destruct (Mem.to_int _ m) eqn:?; ss; clarify.
+    - hexploit match_to_int; et. i. rewrite H in Heqo. clarify.
+    - hexploit match_to_int; et. i. rewrite H in Heqo. clarify.
+  Qed.
+
+  (* Lemma ip_comm m c b ofs ofs' i i' :
+    Mem.to_int (Vptr b ofs) m = Some (Vlong i) ->
+    Mem.to_ptr (Vlong i') m = Some (Vptr b ofs') ->
+    Int64.cmpu c i i' = Ptrofs.cmpu c ofs ofs'.
+  Proof.
+    i. unfold Mem.to_int, Mem.to_ptr, Mem.ptr2int_v, Mem.ptr2int in *. des_ifs.
+    unfold Mem.denormalize in Heq1. apply Maps.PTree.gselectf in Heq1.
+    des. unfold Mem.denormalize_aux, Mem.is_valid, Mem.addr_is_in_block in Heq2.
+    des_ifs; bsimpl; clarify. change Ptrofs.modulus with (Ptrofs.max_unsigned + 1)%Z in Heq1.
+    destruct c; ss; unfold Int64.eq, Ptrofs.eq, Int64.ltu, Ptrofs.ltu.
+    all: rewrite Ptrofs.unsigned_repr; try nia.
+    - des_ifs; exfalso; apply n.
+      +  *)
+
+  Lemma step_cmp_ptr pstate f_table modl cprog sk tge le tle e te m tm
+    (PSTATE: pstate "Mem"%string = m↑)
+    (EQ: f_table = (ModL.add Mem modl).(ModL.enclose))
+    (ME: match_e sk tge e te)
+    (MLE: match_le sk tge le tle)
+    (MGE: match_ge sk tge)
+    (MM: match_mem sk tge m tm)
+    c v1 v2
     tf tcode tcont ktr bflag r mn
     (NEXT: forall b,
-            (Mem.weak_valid_pointer tm (map_blk sk tge blk) ofs = b) ->
+          Cop.cmp_ptr_join_common tm c (map_val sk tge v1) (map_val sk tge v2) = Some (Val.of_bool b) ->
             paco4
               (_sim (ModL.compile (ModL.add Mem modl)) (semantics2 cprog)) r true bflag
               (ktr (pstate, b))
@@ -320,17 +587,295 @@ Section PROOF.
       (`r0: (p_state * bool) <- 
         (EventsL.interp_Es
           (prog f_table)
-          (transl_all mn (weak_valid_pointer_c blk ofs)) 
+          (transl_all mn (ccallU "cmp_ptr" (c, v1, v2))) 
           pstate);; ktr r0)
       (State tf tcode tcont te tle tm).
   Proof.
-    unfold weak_valid_pointer_c, ccallU. sim_red. sim_tau. ss. unfold valid_pointerF. sim_red. 
-    repeat (sim_tau; sim_red). rewrite PSTATE. sim_red. repeat (sim_tau; sim_red).
-    unfold valid_pointerF. sim_red. repeat (sim_tau; sim_red). rewrite PSTATE.
-    sim_red. repeat (sim_tau; sim_red). eapplyf NEXT; et.
+    unfold ccallU. step. ss. unfold cmp_ptrF. step. rewrite PSTATE. rewrite Any.upcast_downcast.
+    step. unfold cmp_ptr. remove_UBcase.
+    - unfold cmp_ptr_join. unfold cmp_ptr. remove_UBcase. remove_UBcase.
+    - sim_tau. sim_red. eapplyf NEXT. ss.
+    - remove_UBcase. unfold unwrapU. remove_UBcase. sim_tau. step. rewrite Any.upcast_downcast. step.
+      eapplyf NEXT. unfold Cop.cmp_ptr. des_ifs. ss. erewrite match_valid_pointer; et.
+      erewrite match_valid_pointer; et. des_ifs; ss; clarify. rewrite Heq3. ss.
+    - unfold cmp_ptr_join. unfold cmp_ptr. remove_UBcase.
+      unfold Val.cmplu_bool. destruct IntPtrRel.to_ptr_val eqn:?; clarify.
+      all: try solve [unfold IntPtrRel.to_ptr_val, Mem.to_ptr in *; des_ifs].
+      + remove_UBcase. sim_tau. step. eapplyf NEXT. hexploit match_to_int_val; et. i.
+        unfold Cop.cmp_ptr_join, Cop.cmp_ptr, Val.cmplu_bool.
+        ss. rewrite Heq0. ss. unfold IntPtrRel.to_ptr_val, Mem.to_ptr. des_ifs.
+        all: try solve [ss; clarify; unfold Val.of_bool in *; des_ifs].
+        all: try solve [unfold Val.cmp_different_blocks in *; des_ifs].
+        all: try solve [ss; clarify; hexploit match_mem_denormalize_rev; et; i; unfold IntPtrRel.to_ptr_val, Mem.to_ptr in Heqv; des_ifs].
+        all: try solve [ss; clarify; rewrite H0; hexploit Int.eq_spec; rewrite Heq4; i; clarify].
+        destruct c; clarify.
+        * hexploit (IntPtrRel.cmplu_no_angelic tm Ceq (Vlong i) (Vptr (map_blk sk tge b) i0) false).
+          { unfold IntPtrRel.to_ptr_val. ss. rewrite Heq8. rewrite Heq. rewrite Heq0.
+            ss. clarify. bsimpl. des. rewrite Heq7. rewrite Heq1. ss. destruct eq_block; clarify. }
+          { rewrite Heq5. ss. }
+          i. red in H. ss. rewrite <- H in *. ss. rewrite Heq1 in Heq3. clarify.
+        * hexploit (IntPtrRel.cmplu_no_angelic tm Cne (Vlong i) (Vptr (map_blk sk tge b) i0) true).
+          { unfold IntPtrRel.to_ptr_val. ss. rewrite Heq8. rewrite Heq. rewrite Heq0.
+            ss. clarify. bsimpl. des. rewrite Heq7. rewrite Heq1. ss. destruct eq_block; clarify. }
+          { rewrite Heq5. ss. }
+          i. red in H. ss. rewrite <- H in *. ss. rewrite Heq1 in Heq3. clarify.
+      + ss. destruct IntPtrRel.to_int_val eqn:?; clarify.
+        all: try solve [unfold IntPtrRel.to_int_val, Mem.to_int, Mem.ptr2int_v in *; des_ifs].
+        * destruct eq_block.
+          { remove_UBcase. sim_tau. step. eapplyf NEXT. unfold Cop.cmp_ptr_join, Cop.cmp_ptr, Val.cmplu_bool.
+            ss. rewrite Heq0. ss. hexploit match_to_ptr_val; et. i. ss. rewrite H.
+            destruct eq_block; clarify.
+            erewrite <- (@match_valid_pointer m) in Heq2; et.
+            erewrite <- (@match_valid_pointer m) in Heq2; et.
+            erewrite <- (@match_valid_pointer m) in Heq2; et.
+            erewrite <- (@match_valid_pointer m) in Heq2; et. rewrite Heq2.
+            ss. destruct Val.of_bool eqn:?; clarify.
+            all: try solve [unfold Val.of_bool in *; des_ifs].
+            unfold IntPtrRel.to_int_val, Mem.to_int, Mem.ptr2int_v, Mem.ptr2int.
+            dup H. unfold IntPtrRel.to_ptr_val, Mem.to_ptr in H0. des_ifs.
+            all: try solve [ss; unfold Val.of_bool in *; des_ifs].
+            inv MM. rewrite <- MEM_CONC in Heq6.
+            unfold IntPtrRel.to_int_val, Mem.to_int, Mem.ptr2int_v, Mem.ptr2int in Heqv0.
+            des_ifs. }
+          remove_UBcase. sim_tau. step. eapplyf NEXT. unfold Cop.cmp_ptr_join, Cop.cmp_ptr, Val.cmplu_bool.
+          ss. rewrite Heq0. ss. hexploit match_to_ptr_val; et. i. ss. rewrite H.
+          destruct eq_block. { hexploit map_blk_inj; et. clarify. }
+          erewrite <- (@match_valid_pointer m) in Heq2; et.
+          erewrite <- (@match_valid_pointer m) in Heq2; et.
+          rewrite Heq2. rewrite Heq1. ss. des_ifs; ss.
+          all: try solve [unfold Val.of_bool in *; des_ifs].
+          unfold IntPtrRel.to_int_val, Mem.to_int, Mem.ptr2int_v, Mem.ptr2int in Heq6. des_ifs.
+          inv MM. rewrite <- MEM_CONC in Heq7.
+          unfold IntPtrRel.to_int_val, Mem.to_int, Mem.ptr2int_v, Mem.ptr2int in Heqv0.
+          des_ifs.
+        * destruct eq_block.
+          { remove_UBcase; sim_tau; sim_red; eapplyf NEXT.
+            - unfold Cop.cmp_ptr_join, Cop.cmp_ptr, Val.cmplu_bool.
+              ss. rewrite Heq0. ss. hexploit match_to_ptr_val; et. i. ss. rewrite H.
+              hexploit match_to_int_val; et. i. ss.
+              destruct eq_block; clarify.
+              erewrite <- (@match_valid_pointer m) in Heq3; et.
+              erewrite <- (@match_valid_pointer m) in Heq3; et.
+              erewrite <- (@match_valid_pointer m) in Heq3; et.
+              erewrite <- (@match_valid_pointer m) in Heq3; et.
+              rewrite Heq3. ss.
+              destruct Val.of_bool eqn:?; clarify.
+              all: try solve [unfold Val.of_bool in *; des_ifs].
+              rewrite H0. ss.
+              hexploit (IntPtrRel.cmplu_no_angelic tm c (Vlong i) (Vptr (map_blk sk tge b) i0) (Ptrofs.cmpu c i1 i0)).
+              { rewrite H. ss. des_ifs. }
+              { rewrite H0. ss. }
+              i. red in H1. rewrite <- H1. rewrite Heqv1. rewrite Int.eq_true. et.
+            - unfold Cop.cmp_ptr_join, Cop.cmp_ptr, Val.cmplu_bool.
+              ss. rewrite Heq0. ss. hexploit match_to_ptr_val; et. i. ss. rewrite H.
+              hexploit match_to_int_val; et. i. ss.
+              destruct eq_block; clarify.
+              erewrite <- (@match_valid_pointer m) in Heq2; et.
+              erewrite <- (@match_valid_pointer m) in Heq2; et.
+              erewrite <- (@match_valid_pointer m) in Heq2; et.
+              erewrite <- (@match_valid_pointer m) in Heq2; et.
+              rewrite Heq2. ss.
+              destruct Val.of_bool eqn:?; clarify.
+              all: try solve [unfold Val.of_bool in *; des_ifs].
+              rewrite H0. ss. rewrite Heqv1. et. }
+          remove_UBcase; sim_tau; sim_red; eapplyf NEXT.
+          { unfold Cop.cmp_ptr_join, Cop.cmp_ptr, Val.cmplu_bool.
+            ss. rewrite Heq0. ss. hexploit match_to_ptr_val; et. i. ss. rewrite H.
+            hexploit match_to_int_val; et. i. ss.
+            destruct eq_block. { hexploit map_blk_inj; et. i. clarify. }
+            erewrite <- (@match_valid_pointer m) in Heq3; et.
+            erewrite <- (@match_valid_pointer m) in Heq3; et.
+            rewrite Heq3. rewrite Heq1. ss.
+            destruct Val.of_bool eqn:?; clarify.
+            all: try solve [unfold Val.of_bool in *; des_ifs].
+            rewrite H0. ss. apply Bool.eqb_prop in Heq2. rewrite <- Heq2.
+            rewrite Heqv1. rewrite Int.eq_true. et. }
+          { unfold Cop.cmp_ptr_join, Cop.cmp_ptr, Val.cmplu_bool.
+            ss. rewrite Heq0. ss. hexploit match_to_ptr_val; et. i. ss. rewrite H.
+            hexploit match_to_int_val; et. i. ss.
+            destruct eq_block. { hexploit map_blk_inj; et. i. clarify. }
+            erewrite <- (@match_valid_pointer m) in Heq2; et.
+            erewrite <- (@match_valid_pointer m) in Heq2; et.
+            rewrite Heq2. rewrite Heq1. ss. rewrite H0. ss.
+            destruct Val.of_bool eqn:?; clarify.
+            all: try solve [unfold Val.of_bool in *; des_ifs]. }
+          { unfold Cop.cmp_ptr_join, Cop.cmp_ptr, Val.cmplu_bool.
+            ss. rewrite Heq0. ss. hexploit match_to_ptr_val; et. i. ss. rewrite H.
+            hexploit match_to_int_val; et. i. ss.
+            destruct eq_block. { hexploit map_blk_inj; et. i. clarify. }
+            erewrite <- (@match_valid_pointer m) in Heq2; et.
+            erewrite <- (@match_valid_pointer m) in Heq2; et.
+            rewrite Heq2. ss. rewrite H0. ss.
+            destruct Val.of_bool eqn:?; clarify.
+            all: try solve [unfold Val.of_bool in *; des_ifs]. }
+    - unfold cmp_ptr_join. unfold cmp_ptr. remove_UBcase. remove_UBcase.
+      sim_tau. sim_red. unfold Val.cmplu_bool in *. des_ifs.
+    - rewrite Heq. ss. remove_UBcase. unfold unwrapU. remove_UBcase. sim_tau.
+      step. rewrite Any.upcast_downcast. step. eapplyf NEXT.
+      unfold Cop.cmp_ptr, Val.cmplu_bool. rewrite Heq.
+      erewrite match_valid_pointer; et.
+      erewrite match_valid_pointer; et. rewrite Heq2. ss. des_ifs.
+      rewrite Heq3. ss.
+    - unfold cmp_ptr_join. unfold cmp_ptr. remove_UBcase.
+      unfold Val.cmplu_bool. destruct IntPtrRel.to_ptr_val eqn:?; clarify.
+      all: try solve [unfold IntPtrRel.to_ptr_val, Mem.to_ptr in *; des_ifs].
+      + remove_UBcase. sim_tau. step. eapplyf NEXT. hexploit match_to_int_val; et. i.
+        unfold Cop.cmp_ptr_join, Cop.cmp_ptr, Val.cmplu_bool.
+        ss. rewrite Heq0. ss. unfold IntPtrRel.to_ptr_val, Mem.to_ptr. des_ifs.
+        all: try solve [ss; clarify; unfold Val.of_bool in *; des_ifs].
+        all: try solve [unfold Val.cmp_different_blocks in *; des_ifs].
+        all: try solve [ss; clarify; hexploit match_mem_denormalize_rev; et; i; unfold IntPtrRel.to_ptr_val, Mem.to_ptr in Heqv; des_ifs].
+        all: try solve [ss; clarify; rewrite H0; hexploit Int.eq_spec; rewrite Heq4; i; clarify].
+        destruct c; clarify.
+        * hexploit (IntPtrRel.cmplu_no_angelic tm Ceq (Vptr (map_blk sk tge b) i) (Vlong i0) false).
+          { unfold IntPtrRel.to_ptr_val. ss. rewrite Heq8. rewrite Heq. rewrite Heq0.
+            ss. clarify. bsimpl. des. rewrite Heq7. rewrite Heq1. ss. destruct eq_block; clarify. }
+          { rewrite Heq5. ss. }
+          i. red in H. ss. rewrite <- H in *. ss. rewrite Heq1 in Heq3. clarify.
+        * hexploit (IntPtrRel.cmplu_no_angelic tm Cne (Vptr (map_blk sk tge b) i) (Vlong i0) true).
+          { unfold IntPtrRel.to_ptr_val. ss. rewrite Heq8. rewrite Heq. rewrite Heq0.
+            ss. clarify. bsimpl. des. rewrite Heq7. rewrite Heq1. ss. destruct eq_block; clarify. }
+          { rewrite Heq5. ss. }
+          i. red in H. ss. rewrite <- H in *. ss. rewrite Heq1 in Heq3. clarify.
+      + ss. destruct IntPtrRel.to_int_val eqn:?; clarify.
+        all: try solve [unfold IntPtrRel.to_int_val, Mem.to_int, Mem.ptr2int_v in *; des_ifs].
+        * destruct eq_block.
+          { remove_UBcase. sim_tau. step. eapplyf NEXT. unfold Cop.cmp_ptr_join, Cop.cmp_ptr, Val.cmplu_bool.
+            ss. rewrite Heq0. ss. hexploit match_to_ptr_val; et. i. ss. rewrite H.
+            destruct eq_block; clarify.
+            erewrite <- (@match_valid_pointer m) in Heq2; et.
+            erewrite <- (@match_valid_pointer m) in Heq2; et.
+            erewrite <- (@match_valid_pointer m) in Heq2; et.
+            erewrite <- (@match_valid_pointer m) in Heq2; et. rewrite Heq2.
+            ss. destruct Val.of_bool eqn:?; clarify.
+            all: try solve [unfold Val.of_bool in *; des_ifs].
+            unfold IntPtrRel.to_int_val, Mem.to_int, Mem.ptr2int_v, Mem.ptr2int.
+            dup H. unfold IntPtrRel.to_ptr_val, Mem.to_ptr in H0. des_ifs.
+            all: try solve [ss; unfold Val.of_bool in *; des_ifs].
+            inv MM. rewrite <- MEM_CONC in Heq6.
+            unfold IntPtrRel.to_int_val, Mem.to_int, Mem.ptr2int_v, Mem.ptr2int in Heqv0.
+            des_ifs. }
+          remove_UBcase. sim_tau. step. eapplyf NEXT. unfold Cop.cmp_ptr_join, Cop.cmp_ptr, Val.cmplu_bool.
+          ss. rewrite Heq0. ss. hexploit match_to_ptr_val; et. i. ss. rewrite H.
+          destruct eq_block. { hexploit map_blk_inj; et. clarify. }
+          erewrite <- (@match_valid_pointer m) in Heq2; et.
+          erewrite <- (@match_valid_pointer m) in Heq2; et.
+          rewrite Heq2. rewrite Heq1. ss. des_ifs; ss.
+          all: try solve [unfold Val.of_bool in *; des_ifs].
+          unfold IntPtrRel.to_int_val, Mem.to_int, Mem.ptr2int_v, Mem.ptr2int in Heq6. des_ifs.
+          inv MM. rewrite <- MEM_CONC in Heq7.
+          unfold IntPtrRel.to_int_val, Mem.to_int, Mem.ptr2int_v, Mem.ptr2int in Heqv0.
+          des_ifs.
+        * destruct eq_block.
+          { remove_UBcase; sim_tau; sim_red; eapplyf NEXT.
+            - unfold Cop.cmp_ptr_join, Cop.cmp_ptr, Val.cmplu_bool.
+              ss. rewrite Heq0. ss. hexploit match_to_ptr_val; et. i. ss. rewrite H.
+              hexploit match_to_int_val; et. i. ss.
+              destruct eq_block; clarify.
+              erewrite <- (@match_valid_pointer m) in Heq3; et.
+              erewrite <- (@match_valid_pointer m) in Heq3; et.
+              erewrite <- (@match_valid_pointer m) in Heq3; et.
+              erewrite <- (@match_valid_pointer m) in Heq3; et.
+              rewrite Heq3. ss.
+              destruct Val.of_bool eqn:?; clarify.
+              all: try solve [unfold Val.of_bool in *; des_ifs].
+              rewrite H0. ss.
+              hexploit (IntPtrRel.cmplu_no_angelic tm c (Vptr (map_blk sk tge b0) i) (Vlong i0) (Ptrofs.cmpu c i i1)).
+              { rewrite H. ss. des_ifs. }
+              { rewrite H0. ss. }
+              i. red in H1. rewrite <- H1. rewrite Heqv1. rewrite Int.eq_true. et.
+            - unfold Cop.cmp_ptr_join, Cop.cmp_ptr, Val.cmplu_bool.
+              ss. rewrite Heq0. ss. hexploit match_to_ptr_val; et. i. ss. rewrite H.
+              hexploit match_to_int_val; et. i. ss.
+              destruct eq_block; clarify.
+              erewrite <- (@match_valid_pointer m) in Heq2; et.
+              erewrite <- (@match_valid_pointer m) in Heq2; et.
+              erewrite <- (@match_valid_pointer m) in Heq2; et.
+              erewrite <- (@match_valid_pointer m) in Heq2; et.
+              rewrite Heq2. ss.
+              destruct Val.of_bool eqn:?; clarify.
+              all: try solve [unfold Val.of_bool in *; des_ifs].
+              rewrite H0. ss. rewrite Heqv1. et. }
+          remove_UBcase; sim_tau; sim_red; eapplyf NEXT.
+          { unfold Cop.cmp_ptr_join, Cop.cmp_ptr, Val.cmplu_bool.
+            ss. rewrite Heq0. ss. hexploit match_to_ptr_val; et. i. ss. rewrite H.
+            hexploit match_to_int_val; et. i. ss.
+            destruct eq_block. { hexploit map_blk_inj; et. i. clarify. }
+            erewrite <- (@match_valid_pointer m) in Heq3; et.
+            erewrite <- (@match_valid_pointer m) in Heq3; et.
+            rewrite Heq3. rewrite Heq1. ss.
+            destruct Val.of_bool eqn:?; clarify.
+            all: try solve [unfold Val.of_bool in *; des_ifs].
+            rewrite H0. ss. apply Bool.eqb_prop in Heq2. rewrite <- Heq2.
+            rewrite Heqv1. rewrite Int.eq_true. et. }
+          { unfold Cop.cmp_ptr_join, Cop.cmp_ptr, Val.cmplu_bool.
+            ss. rewrite Heq0. ss. hexploit match_to_ptr_val; et. i. ss. rewrite H.
+            hexploit match_to_int_val; et. i. ss.
+            destruct eq_block. { hexploit map_blk_inj; et. i. clarify. }
+            erewrite <- (@match_valid_pointer m) in Heq2; et.
+            erewrite <- (@match_valid_pointer m) in Heq2; et.
+            rewrite Heq2. rewrite Heq1. ss. rewrite H0. ss.
+            destruct Val.of_bool eqn:?; clarify.
+            all: try solve [unfold Val.of_bool in *; des_ifs]. }
+          { unfold Cop.cmp_ptr_join, Cop.cmp_ptr, Val.cmplu_bool.
+            ss. rewrite Heq0. ss. hexploit match_to_ptr_val; et. i. ss. rewrite H.
+            hexploit match_to_int_val; et. i. ss.
+            destruct eq_block. { hexploit map_blk_inj; et. i. clarify. }
+            erewrite <- (@match_valid_pointer m) in Heq2; et.
+            erewrite <- (@match_valid_pointer m) in Heq2; et.
+            rewrite Heq2. ss. rewrite H0. ss.
+            destruct Val.of_bool eqn:?; clarify.
+            all: try solve [unfold Val.of_bool in *; des_ifs]. }
+    - ss. remove_UBcase.
+      + sim_tau. step. eapplyf NEXT. unfold Cop.cmp_ptr. unfold Val.cmplu_bool.
+        erewrite (@match_valid_pointer m); et.
+        erewrite (@match_valid_pointer m); et.
+        erewrite (@match_valid_pointer m); et.
+        erewrite (@match_valid_pointer m); et.
+        rewrite Heq1.
+        destruct eq_block; clarify.
+      + unfold unwrapU. remove_UBcase. sim_tau. step. rewrite Any.upcast_downcast.
+        step. eapplyf NEXT. unfold Cop.cmp_ptr. unfold Val.cmplu_bool.
+        erewrite (@match_valid_pointer m); et.
+        erewrite (@match_valid_pointer m); et.
+        erewrite (@match_valid_pointer m); et.
+        rewrite Heq1. destruct eq_block. { hexploit map_blk_inj; et. clarify. }
+        des_ifs. rewrite Heq2. ss.
+  Qed.
+
+        
+  Lemma step_non_null_ptr pstate f_table modl cprog sk tge le tle e te m tm
+    (PSTATE: pstate "Mem"%string = m↑)
+    (EQ: f_table = (ModL.add Mem modl).(ModL.enclose))
+    (ME: match_e sk tge e te)
+    (MLE: match_le sk tge le tle)
+    (MM: match_mem sk tge m tm)
+    blk ofs
+    tf tcode tcont ktr bflag r mn
+    (NEXT: Mem.weak_valid_pointer tm (map_blk sk tge blk) (Ptrofs.unsigned ofs) = true ->
+            paco4
+              (_sim (ModL.compile (ModL.add Mem modl)) (semantics2 cprog)) r true bflag
+              (ktr (pstate, true))
+              (State tf tcode tcont te tle tm))
+:
+    paco4
+      (_sim (ModL.compile (ModL.add Mem modl)) (semantics2 cprog)) r true bflag
+      (`r0: (p_state * bool) <- 
+        (EventsL.interp_Es
+          (prog f_table)
+          (transl_all mn (ccallU "non_null?" (Vptr blk ofs))) 
+          pstate);; ktr r0)
+      (State tf tcode tcont te tle tm).
+  Proof.
+    unfold ccallU. sim_red. sim_tau. ss. sim_red. unfold non_nullF. sim_red. repeat (sim_tau; sim_red).
+    rewrite PSTATE. sim_red. remove_UBcase. repeat (sim_tau; sim_red).
+    eapplyf NEXT; et.
     unfold Mem.weak_valid_pointer, Mem.valid_pointer. inv MM.
-    repeat (match goal with | |- context ctx [ Mem.perm_dec ?x ] => destruct (Mem.perm_dec x) end); et;
-      ss; unfold Mem.perm in *; rewrite <- MEM_PERM in *; contradiction.
+    repeat (match goal with | |- context ctx [ Mem.perm_dec ?x ] => destruct (Mem.perm_dec x) end)
+    ; et; ss; unfold Mem.perm in *; rewrite <- MEM_PERM in *.
+    unfold Mem.weak_valid_pointer, Mem.valid_pointer in Heq.
+    destruct Mem.perm_dec in Heq; clarify.
+    destruct Mem.perm_dec in Heq; clarify.
   Qed.
 
   Lemma step_sem_cast pstate f_table modl cprog sk tge le tle e te m tm
@@ -341,49 +886,50 @@ Section PROOF.
     (MM: match_mem sk tge m tm)
     v ty1 ty2
     tf tcode tcont ktr b r mn
-    (NEXT: forall optv,
-            (optv = None -> Cop.sem_cast (map_val sk tge v) ty1 ty2 tm = None) ->
-            (forall v', optv = Some v' -> Cop.sem_cast (map_val sk tge v) ty1 ty2 tm = Some (map_val sk tge v')) ->
+    (NEXT: forall v',
+            Cop.sem_cast (map_val sk tge v) ty1 ty2 tm = Some (map_val sk tge v') ->
             paco4
               (_sim (ModL.compile (ModL.add Mem modl)) (semantics2 cprog)) r true b
-              (ktr (pstate, optv))
+              (ktr (pstate, v'))
               (State tf tcode tcont te tle tm))
 :
     paco4
       (_sim (ModL.compile (ModL.add Mem modl)) (semantics2 cprog)) r true b
-      (`r0: (p_state * option val) <- 
+      (`r0: (p_state * val) <- 
         (EventsL.interp_Es
           (prog f_table)
           (transl_all mn (sem_cast_c v ty1 ty2)) 
           pstate);; ktr r0)
       (State tf tcode tcont te tle tm).
   Proof.
-    unfold sem_cast_c. des_ifs_safe. des_ifs.
-    all: try solve [sim_red; eapplyf NEXT; i; clarify; ss; unfold Cop.sem_cast; des_ifs].
-    sim_red. eapply step_weak_valid_pointer; et. i. 
-      des_ifs; sim_red; eapplyf NEXT; et; ss; i; clarify;
-       unfold Cop.sem_cast; rewrite Heq1; des_ifs_safe. 
+    unfold sem_cast_c. des_ifs_safe. unfold cast_to_ptr. remove_UBcase.
+    all: try solve [eapplyf NEXT; unfold Cop.sem_cast; des_ifs].
+    all: try solve [unfold unwrapU; remove_UBcase; eapplyf NEXT; unfold Cop.sem_cast; des_ifs; ss; clarify].
+    eapply step_non_null_ptr; et. i. sim_red. eapplyf NEXT; et.
+    unfold Cop.sem_cast. rewrite Heq1; des_ifs_safe.
+    ss. clarify.
   Qed.
 
-  Lemma divide_c_divides a b : (a > 0)%Z -> (divide_c a b = true <-> (a | b)).
+  Lemma divide_c_divides a b : (a > 0)%Z -> (divide_c a b = true <-> (a | b)%Z).
   Proof.
     split; i; unfold divide_c in *.
     - rewrite Z.eqb_eq in H0. econs; et.
     - inv H0. rewrite Z_div_mult; try nia.
   Qed.
 
-  Lemma step_assign_loc pstate f_table modl cprog sk tge le tle e te m tm
+  Lemma step_assign_loc pstate f_table modl cprog sk tge le tle e te m tm ce tce
     (PSTATE: pstate "Mem"%string = m↑)
     (EQ: f_table = (ModL.add Mem modl).(ModL.enclose))
     (MGE: match_ge sk tge)
     (ME: match_e sk tge e te)
     (MLE: match_le sk tge le tle)
+    (MCE: match_ce ce tce)
     (MM: match_mem sk tge m tm)
-    ty blk ofs bf v
-    tf tcode tcont ktr b r mn ce
+    ty vp v
+    tf tcode tcont ktr b r mn
     (NEXT: forall tm' m',
             match_mem sk tge m' tm' ->
-            assign_loc ce ty tm (map_blk sk tge blk) ofs bf (map_val sk tge v) tm' ->
+            assign_loc tce ty tm (map_val sk tge vp) (map_val sk tge v) tm' ->
             paco4
               (_sim (ModL.compile (ModL.add Mem modl)) (semantics2 cprog)) r true b
               (ktr (update pstate "Mem" m'↑, ()))
@@ -394,22 +940,17 @@ Section PROOF.
       (`r0: (p_state * ())<- 
         (EventsL.interp_Es
           (prog f_table)
-          (transl_all mn (assign_loc_c ce ty blk ofs bf v)) 
+          (transl_all mn (assign_loc_c ce ty vp v)) 
           pstate);; ktr r0)
       (State tf tcode tcont te tle tm).
   Proof.
     unfold assign_loc_c. des_ifs; try sim_red; try sim_triggerUB.
-    2,3,6,7 : eapply step_store_bitfield; et; i; sim_red; eapplyf NEXT; et; econs; et.
-    - eapply step_store; et. i. des. eapplyf NEXT; et. econs; et. 
-    - eapply step_loadbytes; et. i. eapply step_storebytes; et. i.
-      eapplyf NEXT; et. destruct (_ && _) eqn: E in Heq0; clarify.
-      apply andb_true_iff in E. des. econs 2; et; i.
-      1,2: rewrite <- divide_c_divides; et; pose proof alignof_blockcopy_pos; et.
-      destruct (_||_) eqn: E1 in Heq1 ; clarify. repeat rewrite orb_true_iff in E1.  
-      des; try nia. left. destruct (b0 =? blk)%positive eqn:E2 in E1; clarify.
-      apply Pos.eqb_neq in E2. red. i. apply E2. eapply map_blk_inj; et; admit "".
-    - eapply step_loadbytes; et. i. eapply step_storebytes; et. i.
-      eapplyf NEXT; et. econs 2; et; i; try nia.
+    - eapply step_store; et. i. eapply NEXT; et. econs; et.
+    - eapply step_memcpy; et. i. sim_red. eapply NEXT; et.
+      inv H. 2:{ econs 3; et. erewrite match_sizeof; et. }
+      erewrite <- !match_sizeof in *; et.
+      erewrite <- !match_alignof_blockcopy in *; et.
+      econs 2; et.
   Qed.
 
   Lemma step_deref_loc pstate f_table modl cprog sk tge le tle e te m tm
@@ -419,10 +960,10 @@ Section PROOF.
     (ME: match_e sk tge e te)
     (MLE: match_le sk tge le tle)
     (MM: match_mem sk tge m tm)
-    ty blk ofs bf
+    ty vp
     tf tcode tcont ktr b r mn
     (NEXT: forall v,
-            deref_loc ty tm (map_blk sk tge blk) ofs bf (map_val sk tge v) ->
+            deref_loc ty tm (map_val sk tge vp) (map_val sk tge v) ->
             paco4
               (_sim (ModL.compile (ModL.add Mem modl)) (semantics2 cprog)) r true b
               (ktr (pstate, v))
@@ -433,16 +974,14 @@ Section PROOF.
       (`r0: (p_state * val) <- 
         (EventsL.interp_Es
           (prog f_table)
-          (transl_all mn (deref_loc_c ty blk ofs bf)) 
+          (transl_all mn (deref_loc_c ty vp)) 
           pstate);; ktr r0)
       (State tf tcode tcont te tle tm).
   Proof.
-    unfold deref_loc_c. destruct bf.
-    - remove_UBcase.
-      + eapply step_load; et. i. eapplyf NEXT; ss; econs; et.
-      + eapplyf NEXT; ss; econs 2; et.
-      + eapplyf NEXT; ss; econs 3; et.
-    - des_ifs; eapply step_load_bitfield; et; i; eapplyf NEXT; econs; ss.
+    unfold deref_loc_c. remove_UBcase.
+    - eapply step_load; et. i. eapplyf NEXT; ss; econs; et.
+    - eapplyf NEXT; ss; econs 2; et.
+    - eapplyf NEXT; ss; econs 3; et.
   Qed.
 
   (* Lemma sk_In sk s n : SkEnv.id2blk (Sk.load_skenv sk) s = Some n -> In s (List.map fst sk).
@@ -462,17 +1001,16 @@ Section PROOF.
     (MM: match_mem sk tge m tm)
     uop v ty 
     tf tcode tcont ktr b r mn
-    (NEXT: forall optv,
-            (optv = None -> Cop.sem_unary_operation uop (map_val sk tge v) ty tm = None) ->
-            (forall v', optv = Some v' -> Cop.sem_unary_operation uop (map_val sk tge v) ty tm = Some (map_val sk tge v')) ->
+    (NEXT: forall v',
+            Cop.sem_unary_operation uop (map_val sk tge v) ty tm = Some (map_val sk tge v') ->
             paco4
               (_sim (ModL.compile (ModL.add Mem modl)) (semantics2 cprog)) r true b
-              (ktr (pstate, optv))
+              (ktr (pstate, v'))
               (State tf tcode tcont te tle tm))
 :
     paco4
       (_sim (ModL.compile (ModL.add Mem modl)) (semantics2 cprog)) r true b
-      (`r0: (p_state * option val) <- 
+      (`r0: (p_state * val) <- 
         (EventsL.interp_Es
           (prog f_table)
           (transl_all mn (unary_op_c uop v ty)) 
@@ -480,787 +1018,266 @@ Section PROOF.
       (State tf tcode tcont te tle tm).
   Proof.
     unfold unary_op_c. des_ifs; sim_red.
-    - unfold bool_val_c. des_ifs.
-      all: try solve [sim_red; eapplyf NEXT; i; clarify; ss; unfold Cop.sem_unary_operation; des_ifs; 
-                unfold Cop.sem_notbool, Cop.bool_val; des_ifs].
-      all: try (unfold Values.Val.of_bool; ss; des_ifs).
-      1,2,4,5: sim_red; eapplyf NEXT; i; clarify; ss; unfold Cop.sem_unary_operation; des_ifs; 
-                unfold Cop.sem_notbool, Cop.bool_val; des_ifs; bsimpl; clarify.
-      sim_red. eapply step_weak_valid_pointer; et. i. 
-      destruct b1; sim_red; eapplyf NEXT; et; i; clarify;
-        unfold Cop.sem_notbool, Cop.bool_val; des_ifs.
-    - eapplyf NEXT; i;
-        unfold Cop.sem_unary_operation, Cop.sem_notint in *; des_ifs; ss; clarify.
-    - eapplyf NEXT; i;
-        unfold Cop.sem_unary_operation, Cop.sem_neg in *; des_ifs; ss; clarify.
-    - eapplyf NEXT; i;
-        unfold Cop.sem_unary_operation, Cop.sem_absfloat in *; des_ifs; ss; clarify.
+    - unfold bool_val_c. remove_UBcase.
+      + apply NEXT. unfold Cop.sem_unary_operation. unfold Cop.sem_notbool. ss. unfold Cop.bool_val. rewrite Heq. ss. unfold Val.of_bool. des_ifs.
+      + apply NEXT. unfold Cop.sem_unary_operation. unfold Cop.sem_notbool. ss. unfold Cop.bool_val. rewrite Heq. ss. unfold Val.of_bool. des_ifs.
+      + eapply step_non_null_ptr; et. i. sim_red. apply NEXT. unfold Cop.sem_unary_operation, Cop.sem_notbool, Cop.bool_val. rewrite Heq. ss. rewrite H. des_ifs.
+      + apply NEXT. unfold Cop.sem_unary_operation. unfold Cop.sem_notbool. ss. unfold Cop.bool_val. rewrite Heq. ss. unfold Val.of_bool. des_ifs.
+      + apply NEXT. unfold Cop.sem_unary_operation. unfold Cop.sem_notbool. ss. unfold Cop.bool_val. rewrite Heq. ss. unfold Val.of_bool. des_ifs.
+    - unfold unwrapU. remove_UBcase. apply NEXT.
+      unfold Cop.sem_unary_operation, Cop.sem_notint in *.
+      des_ifs; ss; clarify.
+    - unfold unwrapU. remove_UBcase. apply NEXT.
+      unfold Cop.sem_unary_operation, Cop.sem_neg in *.
+      des_ifs; ss; clarify.
+    - unfold unwrapU. remove_UBcase. apply NEXT.
+      unfold Cop.sem_unary_operation, Cop.sem_absfloat in *.
+      des_ifs; ss; clarify.
   Qed.
 
-  Lemma step_binary_op pstate f_table modl cprog sk tge ce le tle e te m tm
+  Lemma step_binary_op pstate f_table modl cprog sk tge ce tce le tle e te m tm
     (PSTATE: pstate "Mem"%string = m↑)
     (EQ: f_table = (ModL.add Mem modl).(ModL.enclose))
     (MGE: match_ge sk tge)
     (ME: match_e sk tge e te)
     (MLE: match_le sk tge le tle)
+    (MCE: match_ce ce tce)
     (MM: match_mem sk tge m tm)
     biop v1 ty1 v2 ty2
     tf tcode tcont ktr b r mn
-    (NEXT: forall optv,
-            (optv = None -> Cop.sem_binary_operation ce biop (map_val sk tge v1) ty1 (map_val sk tge v2) ty2 tm = None) ->
-            (forall retv, optv = Some retv -> Cop.sem_binary_operation ce biop (map_val sk tge v1) ty1 (map_val sk tge v2) ty2 tm = Some (map_val sk tge retv)) ->
+    (NEXT: forall v',
+            Cop.sem_binary_operation tce biop (map_val sk tge v1) ty1 (map_val sk tge v2) ty2 tm = Some (map_val sk tge v') ->
             paco4
               (_sim (ModL.compile (ModL.add Mem modl)) (semantics2 cprog)) r true b
-              (ktr (pstate, optv))
+              (ktr (pstate, v'))
               (State tf tcode tcont te tle tm))
 :
     paco4
       (_sim (ModL.compile (ModL.add Mem modl)) (semantics2 cprog)) r true b
-      (`r0: (p_state * option val) <- 
+      (`r0: (p_state * val) <- 
         (EventsL.interp_Es
           (prog f_table)
           (transl_all mn (binary_op_c ce biop v1 ty1 v2 ty2)) 
           pstate);; ktr r0)
       (State tf tcode tcont te tle tm).
   Proof.
-    unfold binary_op_c. des_ifs; unfold sem_add_c, sem_sub_c, sem_mul_c, sem_div_c, sem_mod_c, sem_and_c, sem_or_c, sem_xor_c, Cop.sem_shl, Cop.sem_shr, sem_cmp_c; try sim_red.
-    - des_ifs; try sim_red;
-        try (eapplyf NEXT; i; ss;
-            unfold Cop.sem_add; rewrite Heq; unfold Cop.sem_add_ptr_int, Cop.sem_add_ptr_long in *; 
-            des_ifs; ss; clarify).
-      unfold sem_binarith_c. sim_red. eapply step_sem_cast; et. i. destruct optv; sim_red;
-        try solve [eapplyf NEXT; i; clarify; unfold Cop.sem_binary_operation, Cop.sem_add; rewrite Heq; unfold Cop.sem_binarith;
-                  try (erewrite H by et); try (erewrite H0 by et); try (erewrite H1 by et); try (erewrite H2 by et); ss].
-      eapply step_sem_cast; et. i. destruct optv; try sim_red;
-        try solve [eapplyf NEXT; i; clarify; unfold Cop.sem_binary_operation, Cop.sem_add; rewrite Heq; unfold Cop.sem_binarith;
-                  try (erewrite H by et); try (erewrite H0 by et); try (erewrite H1 by et); try (erewrite H2 by et); ss].
-      des_ifs; sim_red; 
-        eapplyf NEXT; i; clarify; unfold Cop.sem_binary_operation, Cop.sem_add; rewrite Heq; unfold Cop.sem_binarith; 
-          rewrite Heq0 in *; try (erewrite H by et); try (erewrite H0 by et); try (erewrite H1 by et); try (erewrite H2 by et); ss.
-    - des_ifs; try sim_red;
-        try (eapplyf NEXT; i; ss; unfold Cop.sem_sub; rewrite Heq; des_ifs; ss; clarify).
-      + eapply map_blk_inj in e0; et. contradiction.
-      + 
-      unfold sem_binarith_c. sim_red. eapply step_sem_cast; et. i. destruct optv; sim_red;
-        try solve [eapplyf NEXT; i; clarify; unfold Cop.sem_binary_operation, Cop.sem_sub; rewrite Heq; unfold Cop.sem_binarith;
-                  try (erewrite H by et); try (erewrite H0 by et); try (erewrite H1 by et); try (erewrite H2 by et); ss].
-      eapply step_sem_cast; et. i. destruct optv; try sim_red;
-        try solve [eapplyf NEXT; i; clarify; unfold Cop.sem_binary_operation, Cop.sem_sub; rewrite Heq; unfold Cop.sem_binarith;
-                  try (erewrite H by et); try (erewrite H0 by et); try (erewrite H1 by et); try (erewrite H2 by et); ss].
-      des_ifs; sim_red; 
-        eapplyf NEXT; i; clarify; unfold Cop.sem_binary_operation, Cop.sem_sub; rewrite Heq; unfold Cop.sem_binarith; 
-          rewrite Heq0 in *; try (erewrite H by et); try (erewrite H0 by et); try (erewrite H1 by et); try (erewrite H2 by et); ss.
-    - unfold sem_binarith_c. sim_red. eapply step_sem_cast; et. i. destruct optv; sim_red;
-        try solve [eapplyf NEXT; i; clarify; unfold Cop.sem_binary_operation, Cop.sem_mul; unfold Cop.sem_binarith;
-                  try (erewrite H by et); try (erewrite H0 by et); try (erewrite H1 by et); try (erewrite H2 by et); ss].
-      eapply step_sem_cast; et. i. destruct optv; try sim_red;
-        try solve [eapplyf NEXT; i; clarify; unfold Cop.sem_binary_operation, Cop.sem_mul; unfold Cop.sem_binarith;
-                  try (erewrite H by et); try (erewrite H0 by et); try (erewrite H1 by et); try (erewrite H2 by et); ss].
-      des_ifs; sim_red; 
-        eapplyf NEXT; i; clarify; unfold Cop.sem_binary_operation, Cop.sem_mul; unfold Cop.sem_binarith; 
-          rewrite Heq in *; try (erewrite H by et); try (erewrite H0 by et); try (erewrite H1 by et); try (erewrite H2 by et); ss.
-    - unfold sem_binarith_c. sim_red. eapply step_sem_cast; et. i. destruct optv; sim_red;
-        try solve [eapplyf NEXT; i; clarify; unfold Cop.sem_binary_operation, Cop.sem_div; unfold Cop.sem_binarith;
-                  try (erewrite H by et); try (erewrite H0 by et); try (erewrite H1 by et); try (erewrite H2 by et); ss].
-      eapply step_sem_cast; et. i. destruct optv; try sim_red;
-        try solve [eapplyf NEXT; i; clarify; unfold Cop.sem_binary_operation, Cop.sem_div; unfold Cop.sem_binarith;
-                  try (erewrite H by et); try (erewrite H0 by et); try (erewrite H1 by et); try (erewrite H2 by et); ss].
-      des_ifs; sim_red; 
-        eapplyf NEXT; i; clarify; unfold Cop.sem_binary_operation, Cop.sem_div; unfold Cop.sem_binarith; 
-          rewrite Heq in *; try (erewrite H by et); try (erewrite H0 by et); try (erewrite H1 by et); try (erewrite H2 by et); ss;
-            rewrite Heq0; ss.
-    - unfold sem_binarith_c. sim_red. eapply step_sem_cast; et. i. destruct optv; sim_red;
-        try solve [eapplyf NEXT; i; clarify; unfold Cop.sem_binary_operation, Cop.sem_mod; unfold Cop.sem_binarith;
-                  try (erewrite H by et); try (erewrite H0 by et); try (erewrite H1 by et); try (erewrite H2 by et); ss].
-      eapply step_sem_cast; et. i. destruct optv; try sim_red;
-        try solve [eapplyf NEXT; i; clarify; unfold Cop.sem_binary_operation, Cop.sem_mod; unfold Cop.sem_binarith;
-                  try (erewrite H by et); try (erewrite H0 by et); try (erewrite H1 by et); try (erewrite H2 by et); ss].
-      des_ifs; sim_red; 
-        eapplyf NEXT; i; clarify; unfold Cop.sem_binary_operation, Cop.sem_mod; unfold Cop.sem_binarith; 
-          rewrite Heq in *; try (erewrite H by et); try (erewrite H0 by et); try (erewrite H1 by et); try (erewrite H2 by et); ss;
-            rewrite Heq0; ss.
-    - unfold sem_binarith_c. sim_red. eapply step_sem_cast; et. i. destruct optv; sim_red;
-        try solve [eapplyf NEXT; i; clarify; unfold Cop.sem_binary_operation, Cop.sem_and; unfold Cop.sem_binarith;
-                  try (erewrite H by et); try (erewrite H0 by et); try (erewrite H1 by et); try (erewrite H2 by et); ss].
-      eapply step_sem_cast; et. i. destruct optv; try sim_red;
-        try solve [eapplyf NEXT; i; clarify; unfold Cop.sem_binary_operation, Cop.sem_and; unfold Cop.sem_binarith;
-                  try (erewrite H by et); try (erewrite H0 by et); try (erewrite H1 by et); try (erewrite H2 by et); ss].
-      des_ifs; sim_red; 
-        eapplyf NEXT; i; clarify; unfold Cop.sem_binary_operation, Cop.sem_and; unfold Cop.sem_binarith; 
-          rewrite Heq in *; try (erewrite H by et); try (erewrite H0 by et); try (erewrite H1 by et); try (erewrite H2 by et); ss;
-            rewrite Heq0; ss.
-    - unfold sem_binarith_c. sim_red. eapply step_sem_cast; et. i. destruct optv; sim_red;
-        try solve [eapplyf NEXT; i; clarify; unfold Cop.sem_binary_operation, Cop.sem_or; unfold Cop.sem_binarith;
-                  try (erewrite H by et); try (erewrite H0 by et); try (erewrite H1 by et); try (erewrite H2 by et); ss].
-      eapply step_sem_cast; et. i. destruct optv; try sim_red;
-        try solve [eapplyf NEXT; i; clarify; unfold Cop.sem_binary_operation, Cop.sem_or; unfold Cop.sem_binarith;
-                  try (erewrite H by et); try (erewrite H0 by et); try (erewrite H1 by et); try (erewrite H2 by et); ss].
-      des_ifs; sim_red; 
-        eapplyf NEXT; i; clarify; unfold Cop.sem_binary_operation, Cop.sem_or; unfold Cop.sem_binarith; 
-          rewrite Heq in *; try (erewrite H by et); try (erewrite H0 by et); try (erewrite H1 by et); try (erewrite H2 by et); ss;
-            rewrite Heq0; ss.
-    - unfold sem_binarith_c. sim_red. eapply step_sem_cast; et. i. destruct optv; sim_red;
-        try solve [eapplyf NEXT; i; clarify; unfold Cop.sem_binary_operation, Cop.sem_xor; unfold Cop.sem_binarith;
-                  try (erewrite H by et); try (erewrite H0 by et); try (erewrite H1 by et); try (erewrite H2 by et); ss].
-      eapply step_sem_cast; et. i. destruct optv; try sim_red;
-        try solve [eapplyf NEXT; i; clarify; unfold Cop.sem_binary_operation, Cop.sem_xor; unfold Cop.sem_binarith;
-                  try (erewrite H by et); try (erewrite H0 by et); try (erewrite H1 by et); try (erewrite H2 by et); ss].
-      des_ifs; sim_red; 
-        eapplyf NEXT; i; clarify; unfold Cop.sem_binary_operation, Cop.sem_xor; unfold Cop.sem_binarith; 
-          rewrite Heq in *; try (erewrite H by et); try (erewrite H0 by et); try (erewrite H1 by et); try (erewrite H2 by et); ss;
-            rewrite Heq0; ss.
-    - eapplyf NEXT; i; clarify; unfold Cop.sem_binary_operation, Cop.sem_shl; unfold Cop.sem_binarith; 
+    unfold binary_op_c. des_ifs; unfold sem_add_c, sem_sub_c, sem_mul_c, sem_div_c, sem_mod_c, sem_and_c, sem_or_c, sem_xor_c, Cop.sem_shl, Cop.sem_shr, sem_cmp_c.
+    - des_ifs.
+      + unfold sem_add_ptr_int_c. remove_UBcase.
+        all: apply NEXT; erewrite <- match_sizeof; et; unfold Cop.sem_binary_operation, Cop.sem_add, Cop.sem_add_ptr_int; ss; des_ifs.
+      + unfold sem_add_ptr_long_c. remove_UBcase.
+        all: apply NEXT; erewrite <- match_sizeof; et; unfold Cop.sem_binary_operation, Cop.sem_add, Cop.sem_add_ptr_long; ss; des_ifs.
+      + unfold sem_add_ptr_int_c. remove_UBcase.
+        all: apply NEXT; erewrite <- match_sizeof; et; unfold Cop.sem_binary_operation, Cop.sem_add, Cop.sem_add_ptr_int; ss; des_ifs.
+      + unfold sem_add_ptr_long_c. remove_UBcase.
+        all: apply NEXT; erewrite <- match_sizeof; et; unfold Cop.sem_binary_operation, Cop.sem_add, Cop.sem_add_ptr_long; ss; des_ifs.
+      + unfold sem_binarith_c. sim_red. eapply step_sem_cast; et. i. sim_red.
+        eapply step_sem_cast; et. i. remove_UBcase.
+        all: apply NEXT; unfold Cop.sem_binary_operation, Cop.sem_add, Cop.sem_binarith; rewrite Heq; rewrite Heq0; des_ifs.
+    - remove_UBcase.
+      + apply NEXT. erewrite <- match_sizeof; et. unfold Cop.sem_binary_operation, Cop.sem_sub. ss; des_ifs.
+      + apply NEXT. erewrite <- match_sizeof; et. unfold Cop.sem_binary_operation, Cop.sem_sub. ss; des_ifs.
+      + eapply step_sub_ptr; et. i. apply NEXT.
+        erewrite <- match_sizeof in *; et. unfold Cop.sem_binary_operation, Cop.sem_sub. ss; des_ifs.
+        destruct Coqlib.zle; destruct Coqlib.zlt; ss; try nia.
+      + apply NEXT. erewrite <- match_sizeof; et. unfold Cop.sem_binary_operation, Cop.sem_sub. ss; des_ifs.
+      + apply NEXT. erewrite <- match_sizeof; et. unfold Cop.sem_binary_operation, Cop.sem_sub. ss; des_ifs.
+      + unfold sem_binarith_c. sim_red. eapply step_sem_cast; et. i. sim_red.
+        eapply step_sem_cast; et. i. remove_UBcase.
+        all: apply NEXT; unfold Cop.sem_binary_operation, Cop.sem_sub, Cop.sem_binarith; rewrite Heq; rewrite Heq0; des_ifs.
+    - unfold sem_binarith_c. sim_red. eapply step_sem_cast; et. i. sim_red.
+      eapply step_sem_cast; et. i. remove_UBcase.
+      all: apply NEXT; unfold Cop.sem_binary_operation, Cop.sem_mul, Cop.sem_binarith; rewrite Heq; des_ifs.
+    - unfold sem_binarith_c. sim_red. eapply step_sem_cast; et. i. sim_red.
+      eapply step_sem_cast; et. i. remove_UBcase.
+      all: apply NEXT; unfold Cop.sem_binary_operation, Cop.sem_div, Cop.sem_binarith; rewrite Heq; des_ifs.
+    - unfold sem_binarith_c. sim_red. eapply step_sem_cast; et. i. sim_red.
+      eapply step_sem_cast; et. i. remove_UBcase.
+      all: apply NEXT; unfold Cop.sem_binary_operation, Cop.sem_mod, Cop.sem_binarith; rewrite Heq; des_ifs.
+    - unfold sem_binarith_c. sim_red. eapply step_sem_cast; et. i. sim_red.
+      eapply step_sem_cast; et. i. remove_UBcase.
+      all: apply NEXT; unfold Cop.sem_binary_operation, Cop.sem_and, Cop.sem_binarith; rewrite Heq; des_ifs.
+    - unfold sem_binarith_c. sim_red. eapply step_sem_cast; et. i. sim_red.
+      eapply step_sem_cast; et. i. remove_UBcase.
+      all: apply NEXT; unfold Cop.sem_binary_operation, Cop.sem_or, Cop.sem_binarith; rewrite Heq; des_ifs.
+    - unfold sem_binarith_c. sim_red. eapply step_sem_cast; et. i. sim_red.
+      eapply step_sem_cast; et. i. remove_UBcase.
+      all: apply NEXT; unfold Cop.sem_binary_operation, Cop.sem_xor, Cop.sem_binarith; rewrite Heq; des_ifs.
+    - unfold unwrapU. remove_UBcase.
+       eapplyf NEXT. i; clarify; unfold Cop.sem_binary_operation, Cop.sem_shl; unfold Cop.sem_binarith; 
         unfold Cop.sem_shift in *; des_ifs; ss; clarify.
-    - eapplyf NEXT; i; clarify; unfold Cop.sem_binary_operation, Cop.sem_shr; unfold Cop.sem_binarith; 
+    - unfold unwrapU. remove_UBcase.
+      eapplyf NEXT; i; clarify; unfold Cop.sem_binary_operation, Cop.sem_shr; unfold Cop.sem_binarith; 
         unfold Cop.sem_shift in *; des_ifs; ss; clarify.
-    - des_ifs; unfold cmp_ptr_c; try sim_red; des_ifs_safe; 
-        try solve [unfold cmplu_bool_c; des_ifs; try sim_red; try eapplyf NEXT; i; ss; clarify; 
-                    unfold Cop.sem_cmp; rewrite Heq; unfold Cop.cmp_ptr; des_ifs_safe].
-      + unfold cmplu_bool_c; des_ifs; try sim_red;
-          try solve [eapplyf NEXT; i; ss; clarify; unfold Cop.sem_cmp; rewrite Heq; unfold Cop.cmp_ptr; des_ifs_safe].
-          2,3: eapply step_weak_valid_pointer; et; i; des_ifs; sim_red; eapplyf NEXT; i; ss; clarify;
-                unfold Cop.sem_cmp; rewrite Heq; unfold Cop.cmp_ptr; ss; des_ifs_safe; 
-                  unfold Mem.weak_valid_pointer in *; clarify.
-        * eapplyf NEXT; i; ss; clarify. unfold Cop.sem_cmp. rewrite Heq. unfold Cop.cmp_ptr. des_ifs_safe. ss.
-          unfold Val.of_bool. des_ifs.
-        * eapply step_weak_valid_pointer; et. i. sim_red. eapply step_weak_valid_pointer; et. i.
-          des_ifs; sim_red; eapplyf NEXT; i; ss; clarify;
-          unfold Cop.sem_cmp; rewrite Heq; unfold Cop.cmp_ptr; ss; des_ifs_safe; unfold Mem.weak_valid_pointer in *; clarify;
-          unfold Val.of_bool; des_ifs. 
-        * unfold ccallU. sim_red. ss. repeat (sim_tau; sim_red). unfold valid_pointerF. sim_red.
-          repeat (sim_tau; sim_red). rewrite PSTATE. sim_red. repeat (sim_tau; sim_red).
-          unfold valid_pointerF. sim_red.
-          repeat (sim_tau; sim_red). rewrite PSTATE. sim_red. repeat (sim_tau; sim_red).
-          repeat match goal with | |- context [Mem.perm_dec ?x ?y ?z ?w ?a] => destruct (Mem.perm_dec x y z w a) end; sim_red;
-            eapplyf NEXT; i; ss; clarify;
-              unfold Cop.sem_cmp; rewrite Heq; unfold Cop.cmp_ptr; ss; unfold Mem.valid_pointer in *;
-                destruct (eq_block _); des_ifs_safe;
-          try solve [eapply map_blk_inj in e0; et; try contradiction];
-          try solve [repeat (destruct (Mem.perm_dec _) in Heq3); inv MM; unfold Mem.perm in *; ss;
-                      rewrite <- MEM_PERM in *; try contradiction].
-      + unfold cmplu_bool_c; des_ifs; try sim_red;
-          try solve [eapplyf NEXT; i; ss; clarify; unfold Cop.sem_cmp; rewrite Heq; unfold Cop.cmp_ptr; des_ifs_safe].
-          2: eapply step_weak_valid_pointer; et; i; des_ifs; sim_red; eapplyf NEXT; i; ss; clarify;
-                unfold Cop.sem_cmp; rewrite Heq; unfold Cop.cmp_ptr; ss; des_ifs_safe; 
-                  unfold Mem.weak_valid_pointer in *; clarify.
-          eapplyf NEXT; i; ss; clarify;
-            unfold Cop.sem_cmp; rewrite Heq; unfold Cop.cmp_ptr; ss; unfold Mem.valid_pointer in *; des_ifs_safe.
-          unfold Val.of_bool; ss. des_ifs.
-      + unfold cmplu_bool_c; des_ifs; try sim_red;
-          try solve [eapplyf NEXT; i; ss; clarify; unfold Cop.sem_cmp; rewrite Heq; unfold Cop.cmp_ptr; des_ifs_safe].
-          1: eapplyf NEXT; i; ss; clarify; unfold Cop.sem_cmp; rewrite Heq; unfold Cop.cmp_ptr; des_ifs_safe.
-          2: eapply step_weak_valid_pointer; et; i; des_ifs; sim_red; eapplyf NEXT; i; ss; clarify;
-                unfold Cop.sem_cmp; rewrite Heq; unfold Cop.cmp_ptr; ss; des_ifs_safe; 
-                  unfold Mem.weak_valid_pointer in *; clarify.
-          all: unfold Val.of_bool; unfold Val.cmplu_bool; des_ifs; unfold Int64.cmpu; rewrite Heq1; ss.
-      + unfold cmplu_bool_c; des_ifs; try sim_red;
-          try solve [eapplyf NEXT; i; ss; clarify; unfold Cop.sem_cmp; rewrite Heq; unfold Cop.cmp_ptr; des_ifs_safe].
-          2: eapply step_weak_valid_pointer; et; i; des_ifs; sim_red; eapplyf NEXT; i; ss; clarify;
-                unfold Cop.sem_cmp; rewrite Heq; unfold Cop.cmp_ptr; ss; des_ifs_safe; 
-                  unfold Mem.weak_valid_pointer in *; clarify.
-          eapplyf NEXT; i; ss; clarify;
-            unfold Cop.sem_cmp; rewrite Heq; unfold Cop.cmp_ptr; ss; unfold Mem.valid_pointer in *; des_ifs_safe.
-          unfold Val.of_bool; ss. des_ifs.
-      + unfold cmplu_bool_c; des_ifs; try sim_red;
-          try solve [eapplyf NEXT; i; ss; clarify; unfold Cop.sem_cmp; rewrite Heq; unfold Cop.cmp_ptr; des_ifs_safe].
-        * eapply step_weak_valid_pointer; et; i; des_ifs; sim_red; eapplyf NEXT; i; ss; clarify;
-                unfold Cop.sem_cmp; rewrite Heq; unfold Cop.cmp_ptr; ss; des_ifs_safe; 
-                  unfold Mem.weak_valid_pointer in *; clarify.
-        * eapply step_weak_valid_pointer; et. i. sim_red. eapply step_weak_valid_pointer; et. i.
-          des_ifs; sim_red; eapplyf NEXT; i; ss; clarify;
-          unfold Cop.sem_cmp; rewrite Heq; unfold Cop.cmp_ptr; ss; des_ifs_safe; unfold Mem.weak_valid_pointer in *; clarify;
-          unfold Val.of_bool; des_ifs. 
-        * unfold ccallU. sim_red. ss. repeat (sim_tau; sim_red). unfold valid_pointerF. sim_red.
-          repeat (sim_tau; sim_red). rewrite PSTATE. sim_red. repeat (sim_tau; sim_red).
-          unfold valid_pointerF. sim_red.
-          repeat (sim_tau; sim_red). rewrite PSTATE. sim_red. repeat (sim_tau; sim_red).
-          repeat match goal with | |- context [Mem.perm_dec ?x ?y ?z ?w ?a] => destruct (Mem.perm_dec x y z w a) end; sim_red;
-            eapplyf NEXT; i; ss; clarify;
-              unfold Cop.sem_cmp; rewrite Heq; unfold Cop.cmp_ptr; ss; unfold Mem.valid_pointer in *;
-                destruct (eq_block _); des_ifs_safe;
-          try solve [eapply map_blk_inj in e0; et; try contradiction];
-          try solve [repeat (destruct (Mem.perm_dec _) in Heq3); inv MM; unfold Mem.perm in *; ss;
-                      rewrite <- MEM_PERM in *; try contradiction].
-      + unfold cmplu_bool_c; des_ifs; try sim_red;
-          try solve [eapplyf NEXT; i; ss; clarify; unfold Cop.sem_cmp; rewrite Heq; unfold Cop.cmp_ptr; des_ifs_safe].
-          1: eapplyf NEXT; i; ss; clarify; unfold Cop.sem_cmp; rewrite Heq; unfold Cop.cmp_ptr; des_ifs_safe.
-          2: eapply step_weak_valid_pointer; et; i; des_ifs; sim_red; eapplyf NEXT; i; ss; clarify;
-                unfold Cop.sem_cmp; rewrite Heq; unfold Cop.cmp_ptr; ss; des_ifs_safe; 
-                  unfold Mem.weak_valid_pointer in *; clarify.
-          all: unfold Val.of_bool; unfold Val.cmplu_bool; des_ifs; unfold Int64.cmpu; rewrite Heq1; ss.
-      + unfold cmplu_bool_c; des_ifs; try sim_red;
-          try solve [eapplyf NEXT; i; ss; clarify; unfold Cop.sem_cmp; rewrite Heq; unfold Cop.cmp_ptr; des_ifs_safe].
-        * eapply step_weak_valid_pointer; et; i; des_ifs; sim_red; eapplyf NEXT; i; ss; clarify;
-                unfold Cop.sem_cmp; rewrite Heq; unfold Cop.cmp_ptr; ss; des_ifs_safe; 
-                  unfold Mem.weak_valid_pointer in *; clarify.
-        * eapply step_weak_valid_pointer; et. i. sim_red. eapply step_weak_valid_pointer; et. i.
-          des_ifs; sim_red; eapplyf NEXT; i; ss; clarify;
-          unfold Cop.sem_cmp; rewrite Heq; unfold Cop.cmp_ptr; ss; des_ifs_safe; unfold Mem.weak_valid_pointer in *; clarify;
-          unfold Val.of_bool; des_ifs. 
-        * unfold ccallU. sim_red. ss. repeat (sim_tau; sim_red). unfold valid_pointerF. sim_red.
-          repeat (sim_tau; sim_red). rewrite PSTATE. sim_red. repeat (sim_tau; sim_red).
-          unfold valid_pointerF. sim_red.
-          repeat (sim_tau; sim_red). rewrite PSTATE. sim_red. repeat (sim_tau; sim_red).
-          repeat match goal with | |- context [Mem.perm_dec ?x ?y ?z ?w ?a] => destruct (Mem.perm_dec x y z w a) end; sim_red;
-            eapplyf NEXT; i; ss; clarify;
-              unfold Cop.sem_cmp; rewrite Heq; unfold Cop.cmp_ptr; ss; unfold Mem.valid_pointer in *;
-                destruct (eq_block _); des_ifs_safe;
-          try solve [eapply map_blk_inj in e0; et; try contradiction];
-          try solve [repeat (destruct (Mem.perm_dec _) in Heq3); inv MM; unfold Mem.perm in *; ss;
-                      rewrite <- MEM_PERM in *; try contradiction].
-    + unfold sem_binarith_c. sim_red. eapply step_sem_cast; et. i. destruct optv; sim_red;
-        try solve [ eapplyf NEXT; i; clarify; unfold Cop.sem_binary_operation, Cop.sem_cmp; unfold Cop.sem_binarith; rewrite Heq;
-                  try (erewrite H by et); try (erewrite H0 by et); try (erewrite H1 by et); try (erewrite H2 by et); ss].
-      eapply step_sem_cast; et. i. destruct optv; try sim_red;
-        try solve [eapplyf NEXT; i; clarify; unfold Cop.sem_binary_operation, Cop.sem_cmp; unfold Cop.sem_binarith; rewrite Heq;
-                  try (erewrite H by et); try (erewrite H0 by et); try (erewrite H1 by et); try (erewrite H2 by et); ss].
-      des_ifs; sim_red; 
-        eapplyf NEXT; i; clarify; unfold Cop.sem_binary_operation, Cop.sem_cmp; unfold Cop.sem_binarith; 
-          rewrite Heq in *; rewrite Heq0 in *;
-            try (erewrite H by et); try (erewrite H0 by et); try (erewrite H1 by et); try (erewrite H2 by et); ss.
-      all: unfold Val.of_bool; unfold Val.cmplu_bool; des_ifs; unfold Int64.cmpu; rewrite Heq1; ss.
-    - des_ifs; unfold cmp_ptr_c; try sim_red; des_ifs_safe; 
-        try solve [unfold cmplu_bool_c; des_ifs; try sim_red; try eapplyf NEXT; i; ss; clarify; 
-                    unfold Cop.sem_cmp; rewrite Heq; unfold Cop.cmp_ptr; des_ifs_safe].
-      + unfold cmplu_bool_c; des_ifs; try sim_red;
-          try solve [eapplyf NEXT; i; ss; clarify; unfold Cop.sem_cmp; rewrite Heq; unfold Cop.cmp_ptr; des_ifs_safe].
-          2,3: eapply step_weak_valid_pointer; et; i; des_ifs; sim_red; eapplyf NEXT; i; ss; clarify;
-                unfold Cop.sem_cmp; rewrite Heq; unfold Cop.cmp_ptr; ss; des_ifs_safe; 
-                  unfold Mem.weak_valid_pointer in *; clarify.
-        * eapplyf NEXT; i; ss; clarify. unfold Cop.sem_cmp. rewrite Heq. unfold Cop.cmp_ptr. des_ifs_safe. ss.
-          unfold Val.of_bool. des_ifs.
-        * eapply step_weak_valid_pointer; et. i. sim_red. eapply step_weak_valid_pointer; et. i.
-          des_ifs; sim_red; eapplyf NEXT; i; ss; clarify;
-          unfold Cop.sem_cmp; rewrite Heq; unfold Cop.cmp_ptr; ss; des_ifs_safe; unfold Mem.weak_valid_pointer in *; clarify;
-          unfold Val.of_bool; des_ifs. 
-        * unfold ccallU. sim_red. ss. repeat (sim_tau; sim_red). unfold valid_pointerF. sim_red.
-          repeat (sim_tau; sim_red). rewrite PSTATE. sim_red. repeat (sim_tau; sim_red).
-          unfold valid_pointerF. sim_red.
-          repeat (sim_tau; sim_red). rewrite PSTATE. sim_red. repeat (sim_tau; sim_red).
-          repeat match goal with | |- context [Mem.perm_dec ?x ?y ?z ?w ?a] => destruct (Mem.perm_dec x y z w a) end; sim_red;
-            eapplyf NEXT; i; ss; clarify;
-              unfold Cop.sem_cmp; rewrite Heq; unfold Cop.cmp_ptr; ss; unfold Mem.valid_pointer in *;
-                destruct (eq_block _); des_ifs_safe;
-          try solve [eapply map_blk_inj in e0; et; try contradiction];
-          try solve [repeat (destruct (Mem.perm_dec _) in Heq3); inv MM; unfold Mem.perm in *; ss;
-                      rewrite <- MEM_PERM in *; try contradiction].
-      + unfold cmplu_bool_c; des_ifs; try sim_red;
-          try solve [eapplyf NEXT; i; ss; clarify; unfold Cop.sem_cmp; rewrite Heq; unfold Cop.cmp_ptr; des_ifs_safe].
-          2: eapply step_weak_valid_pointer; et; i; des_ifs; sim_red; eapplyf NEXT; i; ss; clarify;
-                unfold Cop.sem_cmp; rewrite Heq; unfold Cop.cmp_ptr; ss; des_ifs_safe; 
-                  unfold Mem.weak_valid_pointer in *; clarify.
-          eapplyf NEXT; i; ss; clarify;
-            unfold Cop.sem_cmp; rewrite Heq; unfold Cop.cmp_ptr; ss; unfold Mem.valid_pointer in *; des_ifs_safe.
-          unfold Val.of_bool; ss. des_ifs.
-      + unfold cmplu_bool_c; des_ifs; try sim_red;
-          try solve [eapplyf NEXT; i; ss; clarify; unfold Cop.sem_cmp; rewrite Heq; unfold Cop.cmp_ptr; des_ifs_safe].
-          1: eapplyf NEXT; i; ss; clarify; unfold Cop.sem_cmp; rewrite Heq; unfold Cop.cmp_ptr; des_ifs_safe.
-          2: eapply step_weak_valid_pointer; et; i; des_ifs; sim_red; eapplyf NEXT; i; ss; clarify;
-                unfold Cop.sem_cmp; rewrite Heq; unfold Cop.cmp_ptr; ss; des_ifs_safe; 
-                  unfold Mem.weak_valid_pointer in *; clarify.
-          all: unfold Val.of_bool; unfold Val.cmplu_bool; des_ifs; unfold Int64.cmpu; rewrite Heq1; ss.
-      + unfold cmplu_bool_c; des_ifs; try sim_red;
-          try solve [eapplyf NEXT; i; ss; clarify; unfold Cop.sem_cmp; rewrite Heq; unfold Cop.cmp_ptr; des_ifs_safe].
-          2: eapply step_weak_valid_pointer; et; i; des_ifs; sim_red; eapplyf NEXT; i; ss; clarify;
-                unfold Cop.sem_cmp; rewrite Heq; unfold Cop.cmp_ptr; ss; des_ifs_safe; 
-                  unfold Mem.weak_valid_pointer in *; clarify.
-          eapplyf NEXT; i; ss; clarify;
-            unfold Cop.sem_cmp; rewrite Heq; unfold Cop.cmp_ptr; ss; unfold Mem.valid_pointer in *; des_ifs_safe.
-          unfold Val.of_bool; ss. des_ifs.
-      + unfold cmplu_bool_c; des_ifs; try sim_red;
-          try solve [eapplyf NEXT; i; ss; clarify; unfold Cop.sem_cmp; rewrite Heq; unfold Cop.cmp_ptr; des_ifs_safe].
-        * eapply step_weak_valid_pointer; et; i; des_ifs; sim_red; eapplyf NEXT; i; ss; clarify;
-                unfold Cop.sem_cmp; rewrite Heq; unfold Cop.cmp_ptr; ss; des_ifs_safe; 
-                  unfold Mem.weak_valid_pointer in *; clarify.
-        * eapply step_weak_valid_pointer; et. i. sim_red. eapply step_weak_valid_pointer; et. i.
-          des_ifs; sim_red; eapplyf NEXT; i; ss; clarify;
-          unfold Cop.sem_cmp; rewrite Heq; unfold Cop.cmp_ptr; ss; des_ifs_safe; unfold Mem.weak_valid_pointer in *; clarify;
-          unfold Val.of_bool; des_ifs. 
-        * unfold ccallU. sim_red. ss. repeat (sim_tau; sim_red). unfold valid_pointerF. sim_red.
-          repeat (sim_tau; sim_red). rewrite PSTATE. sim_red. repeat (sim_tau; sim_red).
-          unfold valid_pointerF. sim_red.
-          repeat (sim_tau; sim_red). rewrite PSTATE. sim_red. repeat (sim_tau; sim_red).
-          repeat match goal with | |- context [Mem.perm_dec ?x ?y ?z ?w ?a] => destruct (Mem.perm_dec x y z w a) end; sim_red;
-            eapplyf NEXT; i; ss; clarify;
-              unfold Cop.sem_cmp; rewrite Heq; unfold Cop.cmp_ptr; ss; unfold Mem.valid_pointer in *;
-                destruct (eq_block _); des_ifs_safe;
-          try solve [eapply map_blk_inj in e0; et; try contradiction];
-          try solve [repeat (destruct (Mem.perm_dec _) in Heq3); inv MM; unfold Mem.perm in *; ss;
-                      rewrite <- MEM_PERM in *; try contradiction].
-      + unfold cmplu_bool_c; des_ifs; try sim_red;
-          try solve [eapplyf NEXT; i; ss; clarify; unfold Cop.sem_cmp; rewrite Heq; unfold Cop.cmp_ptr; des_ifs_safe].
-          1: eapplyf NEXT; i; ss; clarify; unfold Cop.sem_cmp; rewrite Heq; unfold Cop.cmp_ptr; des_ifs_safe.
-          2: eapply step_weak_valid_pointer; et; i; des_ifs; sim_red; eapplyf NEXT; i; ss; clarify;
-                unfold Cop.sem_cmp; rewrite Heq; unfold Cop.cmp_ptr; ss; des_ifs_safe; 
-                  unfold Mem.weak_valid_pointer in *; clarify.
-          all: unfold Val.of_bool; unfold Val.cmplu_bool; des_ifs; unfold Int64.cmpu; rewrite Heq1; ss.
-      + unfold cmplu_bool_c; des_ifs; try sim_red;
-          try solve [eapplyf NEXT; i; ss; clarify; unfold Cop.sem_cmp; rewrite Heq; unfold Cop.cmp_ptr; des_ifs_safe].
-        * eapply step_weak_valid_pointer; et; i; des_ifs; sim_red; eapplyf NEXT; i; ss; clarify;
-                unfold Cop.sem_cmp; rewrite Heq; unfold Cop.cmp_ptr; ss; des_ifs_safe; 
-                  unfold Mem.weak_valid_pointer in *; clarify.
-        * eapply step_weak_valid_pointer; et. i. sim_red. eapply step_weak_valid_pointer; et. i.
-          des_ifs; sim_red; eapplyf NEXT; i; ss; clarify;
-          unfold Cop.sem_cmp; rewrite Heq; unfold Cop.cmp_ptr; ss; des_ifs_safe; unfold Mem.weak_valid_pointer in *; clarify;
-          unfold Val.of_bool; des_ifs. 
-        * unfold ccallU. sim_red. ss. repeat (sim_tau; sim_red). unfold valid_pointerF. sim_red.
-          repeat (sim_tau; sim_red). rewrite PSTATE. sim_red. repeat (sim_tau; sim_red).
-          unfold valid_pointerF. sim_red.
-          repeat (sim_tau; sim_red). rewrite PSTATE. sim_red. repeat (sim_tau; sim_red).
-          repeat match goal with | |- context [Mem.perm_dec ?x ?y ?z ?w ?a] => destruct (Mem.perm_dec x y z w a) end; sim_red;
-            eapplyf NEXT; i; ss; clarify;
-              unfold Cop.sem_cmp; rewrite Heq; unfold Cop.cmp_ptr; ss; unfold Mem.valid_pointer in *;
-                destruct (eq_block _); des_ifs_safe;
-          try solve [eapply map_blk_inj in e0; et; try contradiction];
-          try solve [repeat (destruct (Mem.perm_dec _) in Heq3); inv MM; unfold Mem.perm in *; ss;
-                      rewrite <- MEM_PERM in *; try contradiction].
-    + unfold sem_binarith_c. sim_red. eapply step_sem_cast; et. i. destruct optv; sim_red;
-        try solve [ eapplyf NEXT; i; clarify; unfold Cop.sem_binary_operation, Cop.sem_cmp; unfold Cop.sem_binarith; rewrite Heq;
-                  try (erewrite H by et); try (erewrite H0 by et); try (erewrite H1 by et); try (erewrite H2 by et); ss].
-      eapply step_sem_cast; et. i. destruct optv; try sim_red;
-        try solve [eapplyf NEXT; i; clarify; unfold Cop.sem_binary_operation, Cop.sem_cmp; unfold Cop.sem_binarith; rewrite Heq;
-                  try (erewrite H by et); try (erewrite H0 by et); try (erewrite H1 by et); try (erewrite H2 by et); ss].
-      des_ifs; sim_red; 
-        eapplyf NEXT; i; clarify; unfold Cop.sem_binary_operation, Cop.sem_cmp; unfold Cop.sem_binarith; 
-          rewrite Heq in *; rewrite Heq0 in *;
-            try (erewrite H by et); try (erewrite H0 by et); try (erewrite H1 by et); try (erewrite H2 by et); ss.
-      all: unfold Val.of_bool; unfold Val.cmplu_bool; des_ifs; unfold Int64.cmpu; rewrite Heq1; ss.
-    - des_ifs; unfold cmp_ptr_c; try sim_red; des_ifs_safe; 
-        try solve [unfold cmplu_bool_c; des_ifs; try sim_red; try eapplyf NEXT; i; ss; clarify; 
-                    unfold Cop.sem_cmp; rewrite Heq; unfold Cop.cmp_ptr; des_ifs_safe].
-      + unfold cmplu_bool_c; des_ifs; try sim_red;
-          try solve [eapplyf NEXT; i; ss; clarify; unfold Cop.sem_cmp; rewrite Heq; unfold Cop.cmp_ptr; des_ifs_safe].
-          2,3: eapply step_weak_valid_pointer; et; i; des_ifs; sim_red; eapplyf NEXT; i; ss; clarify;
-                unfold Cop.sem_cmp; rewrite Heq; unfold Cop.cmp_ptr; ss; des_ifs_safe; 
-                  unfold Mem.weak_valid_pointer in *; clarify.
-        * eapplyf NEXT; i; ss; clarify. unfold Cop.sem_cmp. rewrite Heq. unfold Cop.cmp_ptr. des_ifs_safe. ss.
-          unfold Val.of_bool. des_ifs.
-        * eapply step_weak_valid_pointer; et. i. sim_red. eapply step_weak_valid_pointer; et. i.
-          des_ifs; sim_red; eapplyf NEXT; i; ss; clarify;
-          unfold Cop.sem_cmp; rewrite Heq; unfold Cop.cmp_ptr; ss; des_ifs_safe; unfold Mem.weak_valid_pointer in *; clarify;
-          unfold Val.of_bool; des_ifs. 
-        * unfold ccallU. sim_red. ss. repeat (sim_tau; sim_red). unfold valid_pointerF. sim_red.
-          repeat (sim_tau; sim_red). rewrite PSTATE. sim_red. repeat (sim_tau; sim_red).
-          unfold valid_pointerF. sim_red.
-          repeat (sim_tau; sim_red). rewrite PSTATE. sim_red. repeat (sim_tau; sim_red).
-          repeat match goal with | |- context [Mem.perm_dec ?x ?y ?z ?w ?a] => destruct (Mem.perm_dec x y z w a) end; sim_red;
-            eapplyf NEXT; i; ss; clarify;
-              unfold Cop.sem_cmp; rewrite Heq; unfold Cop.cmp_ptr; ss; unfold Mem.valid_pointer in *;
-                destruct (eq_block _); des_ifs_safe;
-          try solve [eapply map_blk_inj in e0; et; try contradiction];
-          repeat (destruct (Mem.perm_dec _)); inv MM; unfold Mem.perm in *; ss.
-      + unfold cmplu_bool_c; des_ifs; try sim_red;
-          try solve [eapplyf NEXT; i; ss; clarify; unfold Cop.sem_cmp; rewrite Heq; unfold Cop.cmp_ptr; des_ifs_safe].
-          2: eapply step_weak_valid_pointer; et; i; des_ifs; sim_red; eapplyf NEXT; i; ss; clarify;
-                unfold Cop.sem_cmp; rewrite Heq; unfold Cop.cmp_ptr; ss; des_ifs_safe; 
-                  unfold Mem.weak_valid_pointer in *; clarify.
-          eapplyf NEXT; i; ss; clarify;
-            unfold Cop.sem_cmp; rewrite Heq; unfold Cop.cmp_ptr; ss; unfold Mem.valid_pointer in *; des_ifs_safe.
-          unfold Val.of_bool; ss. des_ifs.
-      + unfold cmplu_bool_c; des_ifs; try sim_red;
-          try solve [eapplyf NEXT; i; ss; clarify; unfold Cop.sem_cmp; rewrite Heq; unfold Cop.cmp_ptr; des_ifs_safe].
-          1: eapplyf NEXT; i; ss; clarify; unfold Cop.sem_cmp; rewrite Heq; unfold Cop.cmp_ptr; des_ifs_safe.
-          2: eapply step_weak_valid_pointer; et; i; des_ifs; sim_red; eapplyf NEXT; i; ss; clarify;
-                unfold Cop.sem_cmp; rewrite Heq; unfold Cop.cmp_ptr; ss; des_ifs_safe; 
-                  unfold Mem.weak_valid_pointer in *; clarify.
-          all: unfold Val.of_bool; unfold Val.cmplu_bool; des_ifs; unfold Int64.cmpu; rewrite Heq1; ss.
-      + unfold cmplu_bool_c; des_ifs; try sim_red;
-          try solve [eapplyf NEXT; i; ss; clarify; unfold Cop.sem_cmp; rewrite Heq; unfold Cop.cmp_ptr; des_ifs_safe].
-          2: eapply step_weak_valid_pointer; et; i; des_ifs; sim_red; eapplyf NEXT; i; ss; clarify;
-                unfold Cop.sem_cmp; rewrite Heq; unfold Cop.cmp_ptr; ss; des_ifs_safe; 
-                  unfold Mem.weak_valid_pointer in *; clarify.
-          eapplyf NEXT; i; ss; clarify;
-            unfold Cop.sem_cmp; rewrite Heq; unfold Cop.cmp_ptr; ss; unfold Mem.valid_pointer in *; des_ifs_safe.
-          unfold Val.of_bool; ss. des_ifs.
-      + unfold cmplu_bool_c; des_ifs; try sim_red;
-          try solve [eapplyf NEXT; i; ss; clarify; unfold Cop.sem_cmp; rewrite Heq; unfold Cop.cmp_ptr; des_ifs_safe].
-        * eapply step_weak_valid_pointer; et; i; des_ifs; sim_red; eapplyf NEXT; i; ss; clarify;
-                unfold Cop.sem_cmp; rewrite Heq; unfold Cop.cmp_ptr; ss; des_ifs_safe; 
-                  unfold Mem.weak_valid_pointer in *; clarify.
-        * eapply step_weak_valid_pointer; et. i. sim_red. eapply step_weak_valid_pointer; et. i.
-          des_ifs; sim_red; eapplyf NEXT; i; ss; clarify;
-          unfold Cop.sem_cmp; rewrite Heq; unfold Cop.cmp_ptr; ss; des_ifs_safe; unfold Mem.weak_valid_pointer in *; clarify;
-          unfold Val.of_bool; des_ifs. 
-        * unfold ccallU. sim_red. ss. repeat (sim_tau; sim_red). unfold valid_pointerF. sim_red.
-          repeat (sim_tau; sim_red). rewrite PSTATE. sim_red. repeat (sim_tau; sim_red).
-          unfold valid_pointerF. sim_red.
-          repeat (sim_tau; sim_red). rewrite PSTATE. sim_red. repeat (sim_tau; sim_red).
-          repeat match goal with | |- context [Mem.perm_dec ?x ?y ?z ?w ?a] => destruct (Mem.perm_dec x y z w a) end; sim_red;
-            eapplyf NEXT; i; ss; clarify;
-              unfold Cop.sem_cmp; rewrite Heq; unfold Cop.cmp_ptr; ss; unfold Mem.valid_pointer in *;
-                destruct (eq_block _); des_ifs_safe;
-          try solve [eapply map_blk_inj in e0; et; try contradiction];
-          repeat (destruct (Mem.perm_dec _)); inv MM; unfold Mem.perm in *; ss.
-      + unfold cmplu_bool_c; des_ifs; try sim_red;
-          try solve [eapplyf NEXT; i; ss; clarify; unfold Cop.sem_cmp; rewrite Heq; unfold Cop.cmp_ptr; des_ifs_safe].
-          1: eapplyf NEXT; i; ss; clarify; unfold Cop.sem_cmp; rewrite Heq; unfold Cop.cmp_ptr; des_ifs_safe.
-          2: eapply step_weak_valid_pointer; et; i; des_ifs; sim_red; eapplyf NEXT; i; ss; clarify;
-                unfold Cop.sem_cmp; rewrite Heq; unfold Cop.cmp_ptr; ss; des_ifs_safe; 
-                  unfold Mem.weak_valid_pointer in *; clarify.
-          all: unfold Val.of_bool; unfold Val.cmplu_bool; des_ifs; unfold Int64.cmpu; rewrite Heq1; ss.
-      + unfold cmplu_bool_c; des_ifs; try sim_red;
-          try solve [eapplyf NEXT; i; ss; clarify; unfold Cop.sem_cmp; rewrite Heq; unfold Cop.cmp_ptr; des_ifs_safe].
-        * eapply step_weak_valid_pointer; et; i; des_ifs; sim_red; eapplyf NEXT; i; ss; clarify;
-                unfold Cop.sem_cmp; rewrite Heq; unfold Cop.cmp_ptr; ss; des_ifs_safe; 
-                  unfold Mem.weak_valid_pointer in *; clarify.
-        * eapply step_weak_valid_pointer; et. i. sim_red. eapply step_weak_valid_pointer; et. i.
-          des_ifs; sim_red; eapplyf NEXT; i; ss; clarify;
-          unfold Cop.sem_cmp; rewrite Heq; unfold Cop.cmp_ptr; ss; des_ifs_safe; unfold Mem.weak_valid_pointer in *; clarify;
-          unfold Val.of_bool; des_ifs. 
-        * unfold ccallU. sim_red. ss. repeat (sim_tau; sim_red). unfold valid_pointerF. sim_red.
-          repeat (sim_tau; sim_red). rewrite PSTATE. sim_red. repeat (sim_tau; sim_red).
-          unfold valid_pointerF. sim_red.
-          repeat (sim_tau; sim_red). rewrite PSTATE. sim_red. repeat (sim_tau; sim_red).
-          repeat match goal with | |- context [Mem.perm_dec ?x ?y ?z ?w ?a] => destruct (Mem.perm_dec x y z w a) end; sim_red;
-            eapplyf NEXT; i; ss; clarify;
-              unfold Cop.sem_cmp; rewrite Heq; unfold Cop.cmp_ptr; ss; unfold Mem.valid_pointer in *;
-                destruct (eq_block _); des_ifs_safe;
-          try solve [eapply map_blk_inj in e0; et; try contradiction];
-          repeat (destruct (Mem.perm_dec _)); inv MM; unfold Mem.perm in *; ss.
-    + unfold sem_binarith_c. sim_red. eapply step_sem_cast; et. i. destruct optv; sim_red;
-        try solve [ eapplyf NEXT; i; clarify; unfold Cop.sem_binary_operation, Cop.sem_cmp; unfold Cop.sem_binarith; rewrite Heq;
-                  try (erewrite H by et); try (erewrite H0 by et); try (erewrite H1 by et); try (erewrite H2 by et); ss].
-      eapply step_sem_cast; et. i. destruct optv; try sim_red;
-        try solve [eapplyf NEXT; i; clarify; unfold Cop.sem_binary_operation, Cop.sem_cmp; unfold Cop.sem_binarith; rewrite Heq;
-                  try (erewrite H by et); try (erewrite H0 by et); try (erewrite H1 by et); try (erewrite H2 by et); ss].
-      des_ifs; sim_red; 
-        eapplyf NEXT; i; clarify; unfold Cop.sem_binary_operation, Cop.sem_cmp; unfold Cop.sem_binarith; 
-          rewrite Heq in *; rewrite Heq0 in *;
-            try (erewrite H by et); try (erewrite H0 by et); try (erewrite H1 by et); try (erewrite H2 by et); ss.
-      all: unfold Val.of_bool; unfold Val.cmplu_bool; des_ifs; unfold Int64.cmpu; rewrite Heq1; ss.
-    - des_ifs; unfold cmp_ptr_c; try sim_red; des_ifs_safe; 
-        try solve [unfold cmplu_bool_c; des_ifs; try sim_red; try eapplyf NEXT; i; ss; clarify; 
-                    unfold Cop.sem_cmp; rewrite Heq; unfold Cop.cmp_ptr; des_ifs_safe].
-      + unfold cmplu_bool_c; des_ifs; try sim_red;
-          try solve [eapplyf NEXT; i; ss; clarify; unfold Cop.sem_cmp; rewrite Heq; unfold Cop.cmp_ptr; des_ifs_safe].
-          2,3: eapply step_weak_valid_pointer; et; i; des_ifs; sim_red; eapplyf NEXT; i; ss; clarify;
-                unfold Cop.sem_cmp; rewrite Heq; unfold Cop.cmp_ptr; ss; des_ifs_safe; 
-                  unfold Mem.weak_valid_pointer in *; clarify.
-        * eapplyf NEXT; i; ss; clarify. unfold Cop.sem_cmp. rewrite Heq. unfold Cop.cmp_ptr. des_ifs_safe. ss.
-          unfold Val.of_bool. des_ifs.
-        * eapply step_weak_valid_pointer; et. i. sim_red. eapply step_weak_valid_pointer; et. i.
-          des_ifs; sim_red; eapplyf NEXT; i; ss; clarify;
-          unfold Cop.sem_cmp; rewrite Heq; unfold Cop.cmp_ptr; ss; des_ifs_safe; unfold Mem.weak_valid_pointer in *; clarify;
-          unfold Val.of_bool; des_ifs. 
-        * unfold ccallU. sim_red. ss. repeat (sim_tau; sim_red). unfold valid_pointerF. sim_red.
-          repeat (sim_tau; sim_red). rewrite PSTATE. sim_red. repeat (sim_tau; sim_red).
-          unfold valid_pointerF. sim_red.
-          repeat (sim_tau; sim_red). rewrite PSTATE. sim_red. repeat (sim_tau; sim_red).
-          repeat match goal with | |- context [Mem.perm_dec ?x ?y ?z ?w ?a] => destruct (Mem.perm_dec x y z w a) end; sim_red;
-            eapplyf NEXT; i; ss; clarify;
-              unfold Cop.sem_cmp; rewrite Heq; unfold Cop.cmp_ptr; ss; unfold Mem.valid_pointer in *;
-                destruct (eq_block _); des_ifs_safe;
-          try solve [eapply map_blk_inj in e0; et; try contradiction];
-          repeat (destruct (Mem.perm_dec _)); inv MM; unfold Mem.perm in *; ss.
-      + unfold cmplu_bool_c; des_ifs; try sim_red;
-          try solve [eapplyf NEXT; i; ss; clarify; unfold Cop.sem_cmp; rewrite Heq; unfold Cop.cmp_ptr; des_ifs_safe].
-          2: eapply step_weak_valid_pointer; et; i; des_ifs; sim_red; eapplyf NEXT; i; ss; clarify;
-                unfold Cop.sem_cmp; rewrite Heq; unfold Cop.cmp_ptr; ss; des_ifs_safe; 
-                  unfold Mem.weak_valid_pointer in *; clarify.
-          eapplyf NEXT; i; ss; clarify;
-            unfold Cop.sem_cmp; rewrite Heq; unfold Cop.cmp_ptr; ss; unfold Mem.valid_pointer in *; des_ifs_safe.
-          unfold Val.of_bool; ss. des_ifs.
-      + unfold cmplu_bool_c; des_ifs; try sim_red;
-          try solve [eapplyf NEXT; i; ss; clarify; unfold Cop.sem_cmp; rewrite Heq; unfold Cop.cmp_ptr; des_ifs_safe].
-          1: eapplyf NEXT; i; ss; clarify; unfold Cop.sem_cmp; rewrite Heq; unfold Cop.cmp_ptr; des_ifs_safe.
-          2: eapply step_weak_valid_pointer; et; i; des_ifs; sim_red; eapplyf NEXT; i; ss; clarify;
-                unfold Cop.sem_cmp; rewrite Heq; unfold Cop.cmp_ptr; ss; des_ifs_safe; 
-                  unfold Mem.weak_valid_pointer in *; clarify.
-          all: unfold Val.of_bool; unfold Val.cmplu_bool; des_ifs; unfold Int64.cmpu; rewrite Heq1; ss.
-      + unfold cmplu_bool_c; des_ifs; try sim_red;
-          try solve [eapplyf NEXT; i; ss; clarify; unfold Cop.sem_cmp; rewrite Heq; unfold Cop.cmp_ptr; des_ifs_safe].
-          2: eapply step_weak_valid_pointer; et; i; des_ifs; sim_red; eapplyf NEXT; i; ss; clarify;
-                unfold Cop.sem_cmp; rewrite Heq; unfold Cop.cmp_ptr; ss; des_ifs_safe; 
-                  unfold Mem.weak_valid_pointer in *; clarify.
-          eapplyf NEXT; i; ss; clarify;
-            unfold Cop.sem_cmp; rewrite Heq; unfold Cop.cmp_ptr; ss; unfold Mem.valid_pointer in *; des_ifs_safe.
-          unfold Val.of_bool; ss. des_ifs.
-      + unfold cmplu_bool_c; des_ifs; try sim_red;
-          try solve [eapplyf NEXT; i; ss; clarify; unfold Cop.sem_cmp; rewrite Heq; unfold Cop.cmp_ptr; des_ifs_safe].
-        * eapply step_weak_valid_pointer; et; i; des_ifs; sim_red; eapplyf NEXT; i; ss; clarify;
-                unfold Cop.sem_cmp; rewrite Heq; unfold Cop.cmp_ptr; ss; des_ifs_safe; 
-                  unfold Mem.weak_valid_pointer in *; clarify.
-        * eapply step_weak_valid_pointer; et. i. sim_red. eapply step_weak_valid_pointer; et. i.
-          des_ifs; sim_red; eapplyf NEXT; i; ss; clarify;
-          unfold Cop.sem_cmp; rewrite Heq; unfold Cop.cmp_ptr; ss; des_ifs_safe; unfold Mem.weak_valid_pointer in *; clarify;
-          unfold Val.of_bool; des_ifs. 
-        * unfold ccallU. sim_red. ss. repeat (sim_tau; sim_red). unfold valid_pointerF. sim_red.
-          repeat (sim_tau; sim_red). rewrite PSTATE. sim_red. repeat (sim_tau; sim_red).
-          unfold valid_pointerF. sim_red.
-          repeat (sim_tau; sim_red). rewrite PSTATE. sim_red. repeat (sim_tau; sim_red).
-          repeat match goal with | |- context [Mem.perm_dec ?x ?y ?z ?w ?a] => destruct (Mem.perm_dec x y z w a) end; sim_red;
-            eapplyf NEXT; i; ss; clarify;
-              unfold Cop.sem_cmp; rewrite Heq; unfold Cop.cmp_ptr; ss; unfold Mem.valid_pointer in *;
-                destruct (eq_block _); des_ifs_safe;
-          try solve [eapply map_blk_inj in e0; et; try contradiction];
-          repeat (destruct (Mem.perm_dec _)); inv MM; unfold Mem.perm in *; ss.
-      + unfold cmplu_bool_c; des_ifs; try sim_red;
-          try solve [eapplyf NEXT; i; ss; clarify; unfold Cop.sem_cmp; rewrite Heq; unfold Cop.cmp_ptr; des_ifs_safe].
-          1: eapplyf NEXT; i; ss; clarify; unfold Cop.sem_cmp; rewrite Heq; unfold Cop.cmp_ptr; des_ifs_safe.
-          2: eapply step_weak_valid_pointer; et; i; des_ifs; sim_red; eapplyf NEXT; i; ss; clarify;
-                unfold Cop.sem_cmp; rewrite Heq; unfold Cop.cmp_ptr; ss; des_ifs_safe; 
-                  unfold Mem.weak_valid_pointer in *; clarify.
-          all: unfold Val.of_bool; unfold Val.cmplu_bool; des_ifs; unfold Int64.cmpu; rewrite Heq1; ss.
-      + unfold cmplu_bool_c; des_ifs; try sim_red;
-          try solve [eapplyf NEXT; i; ss; clarify; unfold Cop.sem_cmp; rewrite Heq; unfold Cop.cmp_ptr; des_ifs_safe].
-        * eapply step_weak_valid_pointer; et; i; des_ifs; sim_red; eapplyf NEXT; i; ss; clarify;
-                unfold Cop.sem_cmp; rewrite Heq; unfold Cop.cmp_ptr; ss; des_ifs_safe; 
-                  unfold Mem.weak_valid_pointer in *; clarify.
-        * eapply step_weak_valid_pointer; et. i. sim_red. eapply step_weak_valid_pointer; et. i.
-          des_ifs; sim_red; eapplyf NEXT; i; ss; clarify;
-          unfold Cop.sem_cmp; rewrite Heq; unfold Cop.cmp_ptr; ss; des_ifs_safe; unfold Mem.weak_valid_pointer in *; clarify;
-          unfold Val.of_bool; des_ifs. 
-        * unfold ccallU. sim_red. ss. repeat (sim_tau; sim_red). unfold valid_pointerF. sim_red.
-          repeat (sim_tau; sim_red). rewrite PSTATE. sim_red. repeat (sim_tau; sim_red).
-          unfold valid_pointerF. sim_red.
-          repeat (sim_tau; sim_red). rewrite PSTATE. sim_red. repeat (sim_tau; sim_red).
-          repeat match goal with | |- context [Mem.perm_dec ?x ?y ?z ?w ?a] => destruct (Mem.perm_dec x y z w a) end; sim_red;
-            eapplyf NEXT; i; ss; clarify;
-              unfold Cop.sem_cmp; rewrite Heq; unfold Cop.cmp_ptr; ss; unfold Mem.valid_pointer in *;
-                destruct (eq_block _); des_ifs_safe;
-          try solve [eapply map_blk_inj in e0; et; try contradiction];
-          repeat (destruct (Mem.perm_dec _)); inv MM; unfold Mem.perm in *; ss.
-    + unfold sem_binarith_c. sim_red. eapply step_sem_cast; et. i. destruct optv; sim_red;
-        try solve [ eapplyf NEXT; i; clarify; unfold Cop.sem_binary_operation, Cop.sem_cmp; unfold Cop.sem_binarith; rewrite Heq;
-                  try (erewrite H by et); try (erewrite H0 by et); try (erewrite H1 by et); try (erewrite H2 by et); ss].
-      eapply step_sem_cast; et. i. destruct optv; try sim_red;
-        try solve [eapplyf NEXT; i; clarify; unfold Cop.sem_binary_operation, Cop.sem_cmp; unfold Cop.sem_binarith; rewrite Heq;
-                  try (erewrite H by et); try (erewrite H0 by et); try (erewrite H1 by et); try (erewrite H2 by et); ss].
-      des_ifs; sim_red; 
-        eapplyf NEXT; i; clarify; unfold Cop.sem_binary_operation, Cop.sem_cmp; unfold Cop.sem_binarith; 
-          rewrite Heq in *; rewrite Heq0 in *;
-            try (erewrite H by et); try (erewrite H0 by et); try (erewrite H1 by et); try (erewrite H2 by et); ss.
-      all: unfold Val.of_bool; unfold Val.cmplu_bool; des_ifs; unfold Int64.cmpu; rewrite Heq1; ss.
-    - des_ifs; unfold cmp_ptr_c; try sim_red; des_ifs_safe; 
-        try solve [unfold cmplu_bool_c; des_ifs; try sim_red; try eapplyf NEXT; i; ss; clarify; 
-                    unfold Cop.sem_cmp; rewrite Heq; unfold Cop.cmp_ptr; des_ifs_safe].
-      + unfold cmplu_bool_c; des_ifs; try sim_red;
-          try solve [eapplyf NEXT; i; ss; clarify; unfold Cop.sem_cmp; rewrite Heq; unfold Cop.cmp_ptr; des_ifs_safe].
-          2,3: eapply step_weak_valid_pointer; et; i; des_ifs; sim_red; eapplyf NEXT; i; ss; clarify;
-                unfold Cop.sem_cmp; rewrite Heq; unfold Cop.cmp_ptr; ss; des_ifs_safe; 
-                  unfold Mem.weak_valid_pointer in *; clarify.
-        * eapplyf NEXT; i; ss; clarify. unfold Cop.sem_cmp. rewrite Heq. unfold Cop.cmp_ptr. des_ifs_safe. ss.
-          unfold Val.of_bool. des_ifs.
-        * eapply step_weak_valid_pointer; et. i. sim_red. eapply step_weak_valid_pointer; et. i.
-          des_ifs; sim_red; eapplyf NEXT; i; ss; clarify;
-          unfold Cop.sem_cmp; rewrite Heq; unfold Cop.cmp_ptr; ss; des_ifs_safe; unfold Mem.weak_valid_pointer in *; clarify;
-          unfold Val.of_bool; des_ifs. 
-        * unfold ccallU. sim_red. ss. repeat (sim_tau; sim_red). unfold valid_pointerF. sim_red.
-          repeat (sim_tau; sim_red). rewrite PSTATE. sim_red. repeat (sim_tau; sim_red).
-          unfold valid_pointerF. sim_red.
-          repeat (sim_tau; sim_red). rewrite PSTATE. sim_red. repeat (sim_tau; sim_red).
-          repeat match goal with | |- context [Mem.perm_dec ?x ?y ?z ?w ?a] => destruct (Mem.perm_dec x y z w a) end; sim_red;
-            eapplyf NEXT; i; ss; clarify;
-              unfold Cop.sem_cmp; rewrite Heq; unfold Cop.cmp_ptr; ss; unfold Mem.valid_pointer in *;
-                destruct (eq_block _); des_ifs_safe;
-          try solve [eapply map_blk_inj in e0; et; try contradiction];
-          repeat (destruct (Mem.perm_dec _)); inv MM; unfold Mem.perm in *; ss.
-      + unfold cmplu_bool_c; des_ifs; try sim_red;
-          try solve [eapplyf NEXT; i; ss; clarify; unfold Cop.sem_cmp; rewrite Heq; unfold Cop.cmp_ptr; des_ifs_safe].
-          2: eapply step_weak_valid_pointer; et; i; des_ifs; sim_red; eapplyf NEXT; i; ss; clarify;
-                unfold Cop.sem_cmp; rewrite Heq; unfold Cop.cmp_ptr; ss; des_ifs_safe; 
-                  unfold Mem.weak_valid_pointer in *; clarify.
-          eapplyf NEXT; i; ss; clarify;
-            unfold Cop.sem_cmp; rewrite Heq; unfold Cop.cmp_ptr; ss; unfold Mem.valid_pointer in *; des_ifs_safe.
-          unfold Val.of_bool; ss. des_ifs.
-      + unfold cmplu_bool_c; des_ifs; try sim_red;
-          try solve [eapplyf NEXT; i; ss; clarify; unfold Cop.sem_cmp; rewrite Heq; unfold Cop.cmp_ptr; des_ifs_safe].
-          1: eapplyf NEXT; i; ss; clarify; unfold Cop.sem_cmp; rewrite Heq; unfold Cop.cmp_ptr; des_ifs_safe.
-          2: eapply step_weak_valid_pointer; et; i; des_ifs; sim_red; eapplyf NEXT; i; ss; clarify;
-                unfold Cop.sem_cmp; rewrite Heq; unfold Cop.cmp_ptr; ss; des_ifs_safe; 
-                  unfold Mem.weak_valid_pointer in *; clarify.
-          all: unfold Val.of_bool; unfold Val.cmplu_bool; des_ifs; unfold Int64.cmpu; rewrite Heq1; ss.
-      + unfold cmplu_bool_c; des_ifs; try sim_red;
-          try solve [eapplyf NEXT; i; ss; clarify; unfold Cop.sem_cmp; rewrite Heq; unfold Cop.cmp_ptr; des_ifs_safe].
-          2: eapply step_weak_valid_pointer; et; i; des_ifs; sim_red; eapplyf NEXT; i; ss; clarify;
-                unfold Cop.sem_cmp; rewrite Heq; unfold Cop.cmp_ptr; ss; des_ifs_safe; 
-                  unfold Mem.weak_valid_pointer in *; clarify.
-          eapplyf NEXT; i; ss; clarify;
-            unfold Cop.sem_cmp; rewrite Heq; unfold Cop.cmp_ptr; ss; unfold Mem.valid_pointer in *; des_ifs_safe.
-          unfold Val.of_bool; ss. des_ifs.
-      + unfold cmplu_bool_c; des_ifs; try sim_red;
-          try solve [eapplyf NEXT; i; ss; clarify; unfold Cop.sem_cmp; rewrite Heq; unfold Cop.cmp_ptr; des_ifs_safe].
-        * eapply step_weak_valid_pointer; et; i; des_ifs; sim_red; eapplyf NEXT; i; ss; clarify;
-                unfold Cop.sem_cmp; rewrite Heq; unfold Cop.cmp_ptr; ss; des_ifs_safe; 
-                  unfold Mem.weak_valid_pointer in *; clarify.
-        * eapply step_weak_valid_pointer; et. i. sim_red. eapply step_weak_valid_pointer; et. i.
-          des_ifs; sim_red; eapplyf NEXT; i; ss; clarify;
-          unfold Cop.sem_cmp; rewrite Heq; unfold Cop.cmp_ptr; ss; des_ifs_safe; unfold Mem.weak_valid_pointer in *; clarify;
-          unfold Val.of_bool; des_ifs. 
-        * unfold ccallU. sim_red. ss. repeat (sim_tau; sim_red). unfold valid_pointerF. sim_red.
-          repeat (sim_tau; sim_red). rewrite PSTATE. sim_red. repeat (sim_tau; sim_red).
-          unfold valid_pointerF. sim_red.
-          repeat (sim_tau; sim_red). rewrite PSTATE. sim_red. repeat (sim_tau; sim_red).
-          repeat match goal with | |- context [Mem.perm_dec ?x ?y ?z ?w ?a] => destruct (Mem.perm_dec x y z w a) end; sim_red;
-            eapplyf NEXT; i; ss; clarify;
-              unfold Cop.sem_cmp; rewrite Heq; unfold Cop.cmp_ptr; ss; unfold Mem.valid_pointer in *;
-                destruct (eq_block _); des_ifs_safe;
-          try solve [eapply map_blk_inj in e0; et; try contradiction];
-          repeat (destruct (Mem.perm_dec _)); inv MM; unfold Mem.perm in *; ss.
-      + unfold cmplu_bool_c; des_ifs; try sim_red;
-          try solve [eapplyf NEXT; i; ss; clarify; unfold Cop.sem_cmp; rewrite Heq; unfold Cop.cmp_ptr; des_ifs_safe].
-          1: eapplyf NEXT; i; ss; clarify; unfold Cop.sem_cmp; rewrite Heq; unfold Cop.cmp_ptr; des_ifs_safe.
-          2: eapply step_weak_valid_pointer; et; i; des_ifs; sim_red; eapplyf NEXT; i; ss; clarify;
-                unfold Cop.sem_cmp; rewrite Heq; unfold Cop.cmp_ptr; ss; des_ifs_safe; 
-                  unfold Mem.weak_valid_pointer in *; clarify.
-          all: unfold Val.of_bool; unfold Val.cmplu_bool; des_ifs; unfold Int64.cmpu; rewrite Heq1; ss.
-      + unfold cmplu_bool_c; des_ifs; try sim_red;
-          try solve [eapplyf NEXT; i; ss; clarify; unfold Cop.sem_cmp; rewrite Heq; unfold Cop.cmp_ptr; des_ifs_safe].
-        * eapply step_weak_valid_pointer; et; i; des_ifs; sim_red; eapplyf NEXT; i; ss; clarify;
-                unfold Cop.sem_cmp; rewrite Heq; unfold Cop.cmp_ptr; ss; des_ifs_safe; 
-                  unfold Mem.weak_valid_pointer in *; clarify.
-        * eapply step_weak_valid_pointer; et. i. sim_red. eapply step_weak_valid_pointer; et. i.
-          des_ifs; sim_red; eapplyf NEXT; i; ss; clarify;
-          unfold Cop.sem_cmp; rewrite Heq; unfold Cop.cmp_ptr; ss; des_ifs_safe; unfold Mem.weak_valid_pointer in *; clarify;
-          unfold Val.of_bool; des_ifs. 
-        * unfold ccallU. sim_red. ss. repeat (sim_tau; sim_red). unfold valid_pointerF. sim_red.
-          repeat (sim_tau; sim_red). rewrite PSTATE. sim_red. repeat (sim_tau; sim_red).
-          unfold valid_pointerF. sim_red.
-          repeat (sim_tau; sim_red). rewrite PSTATE. sim_red. repeat (sim_tau; sim_red).
-          repeat match goal with | |- context [Mem.perm_dec ?x ?y ?z ?w ?a] => destruct (Mem.perm_dec x y z w a) end; sim_red;
-            eapplyf NEXT; i; ss; clarify;
-              unfold Cop.sem_cmp; rewrite Heq; unfold Cop.cmp_ptr; ss; unfold Mem.valid_pointer in *;
-                destruct (eq_block _); des_ifs_safe;
-          try solve [eapply map_blk_inj in e0; et; try contradiction];
-          repeat (destruct (Mem.perm_dec _)); inv MM; unfold Mem.perm in *; ss.
-    + unfold sem_binarith_c. sim_red. eapply step_sem_cast; et. i. destruct optv; sim_red;
-        try solve [ eapplyf NEXT; i; clarify; unfold Cop.sem_binary_operation, Cop.sem_cmp; unfold Cop.sem_binarith; rewrite Heq;
-                  try (erewrite H by et); try (erewrite H0 by et); try (erewrite H1 by et); try (erewrite H2 by et); ss].
-      eapply step_sem_cast; et. i. destruct optv; try sim_red;
-        try solve [eapplyf NEXT; i; clarify; unfold Cop.sem_binary_operation, Cop.sem_cmp; unfold Cop.sem_binarith; rewrite Heq;
-                  try (erewrite H by et); try (erewrite H0 by et); try (erewrite H1 by et); try (erewrite H2 by et); ss].
-      des_ifs; sim_red; 
-        eapplyf NEXT; i; clarify; unfold Cop.sem_binary_operation, Cop.sem_cmp; unfold Cop.sem_binarith; 
-          rewrite Heq in *; rewrite Heq0 in *;
-            try (erewrite H by et); try (erewrite H0 by et); try (erewrite H1 by et); try (erewrite H2 by et); ss.
-      all: unfold Val.of_bool; unfold Val.cmplu_bool; des_ifs; unfold Int64.cmpu; rewrite Heq1; ss.
-    - des_ifs; unfold cmp_ptr_c; try sim_red; des_ifs_safe; 
-        try solve [unfold cmplu_bool_c; des_ifs; try sim_red; try eapplyf NEXT; i; ss; clarify; 
-                    unfold Cop.sem_cmp; rewrite Heq; unfold Cop.cmp_ptr; des_ifs_safe].
-      + unfold cmplu_bool_c; des_ifs; try sim_red;
-          try solve [eapplyf NEXT; i; ss; clarify; unfold Cop.sem_cmp; rewrite Heq; unfold Cop.cmp_ptr; des_ifs_safe].
-          2,3: eapply step_weak_valid_pointer; et; i; des_ifs; sim_red; eapplyf NEXT; i; ss; clarify;
-                unfold Cop.sem_cmp; rewrite Heq; unfold Cop.cmp_ptr; ss; des_ifs_safe; 
-                  unfold Mem.weak_valid_pointer in *; clarify.
-        * eapplyf NEXT; i; ss; clarify. unfold Cop.sem_cmp. rewrite Heq. unfold Cop.cmp_ptr. des_ifs_safe. ss.
-          unfold Val.of_bool. des_ifs.
-        * eapply step_weak_valid_pointer; et. i. sim_red. eapply step_weak_valid_pointer; et. i.
-          des_ifs; sim_red; eapplyf NEXT; i; ss; clarify;
-          unfold Cop.sem_cmp; rewrite Heq; unfold Cop.cmp_ptr; ss; des_ifs_safe; unfold Mem.weak_valid_pointer in *; clarify;
-          unfold Val.of_bool; des_ifs. 
-        * unfold ccallU. sim_red. ss. repeat (sim_tau; sim_red). unfold valid_pointerF. sim_red.
-          repeat (sim_tau; sim_red). rewrite PSTATE. sim_red. repeat (sim_tau; sim_red).
-          unfold valid_pointerF. sim_red.
-          repeat (sim_tau; sim_red). rewrite PSTATE. sim_red. repeat (sim_tau; sim_red).
-          repeat match goal with | |- context [Mem.perm_dec ?x ?y ?z ?w ?a] => destruct (Mem.perm_dec x y z w a) end; sim_red;
-            eapplyf NEXT; i; ss; clarify;
-              unfold Cop.sem_cmp; rewrite Heq; unfold Cop.cmp_ptr; ss; unfold Mem.valid_pointer in *;
-                destruct (eq_block _); des_ifs_safe;
-          try solve [eapply map_blk_inj in e0; et; try contradiction];
-          repeat (destruct (Mem.perm_dec _)); inv MM; unfold Mem.perm in *; ss.
-      + unfold cmplu_bool_c; des_ifs; try sim_red;
-          try solve [eapplyf NEXT; i; ss; clarify; unfold Cop.sem_cmp; rewrite Heq; unfold Cop.cmp_ptr; des_ifs_safe].
-          2: eapply step_weak_valid_pointer; et; i; des_ifs; sim_red; eapplyf NEXT; i; ss; clarify;
-                unfold Cop.sem_cmp; rewrite Heq; unfold Cop.cmp_ptr; ss; des_ifs_safe; 
-                  unfold Mem.weak_valid_pointer in *; clarify.
-          eapplyf NEXT; i; ss; clarify;
-            unfold Cop.sem_cmp; rewrite Heq; unfold Cop.cmp_ptr; ss; unfold Mem.valid_pointer in *; des_ifs_safe.
-          unfold Val.of_bool; ss. des_ifs.
-      + unfold cmplu_bool_c; des_ifs; try sim_red;
-          try solve [eapplyf NEXT; i; ss; clarify; unfold Cop.sem_cmp; rewrite Heq; unfold Cop.cmp_ptr; des_ifs_safe].
-          1: eapplyf NEXT; i; ss; clarify; unfold Cop.sem_cmp; rewrite Heq; unfold Cop.cmp_ptr; des_ifs_safe.
-          2: eapply step_weak_valid_pointer; et; i; des_ifs; sim_red; eapplyf NEXT; i; ss; clarify;
-                unfold Cop.sem_cmp; rewrite Heq; unfold Cop.cmp_ptr; ss; des_ifs_safe; 
-                  unfold Mem.weak_valid_pointer in *; clarify.
-          all: unfold Val.of_bool; unfold Val.cmplu_bool; des_ifs; unfold Int64.cmpu; rewrite Heq1; ss.
-      + unfold cmplu_bool_c; des_ifs; try sim_red;
-          try solve [eapplyf NEXT; i; ss; clarify; unfold Cop.sem_cmp; rewrite Heq; unfold Cop.cmp_ptr; des_ifs_safe].
-          2: eapply step_weak_valid_pointer; et; i; des_ifs; sim_red; eapplyf NEXT; i; ss; clarify;
-                unfold Cop.sem_cmp; rewrite Heq; unfold Cop.cmp_ptr; ss; des_ifs_safe; 
-                  unfold Mem.weak_valid_pointer in *; clarify.
-          eapplyf NEXT; i; ss; clarify;
-            unfold Cop.sem_cmp; rewrite Heq; unfold Cop.cmp_ptr; ss; unfold Mem.valid_pointer in *; des_ifs_safe.
-          unfold Val.of_bool; ss. des_ifs.
-      + unfold cmplu_bool_c; des_ifs; try sim_red;
-          try solve [eapplyf NEXT; i; ss; clarify; unfold Cop.sem_cmp; rewrite Heq; unfold Cop.cmp_ptr; des_ifs_safe].
-        * eapply step_weak_valid_pointer; et; i; des_ifs; sim_red; eapplyf NEXT; i; ss; clarify;
-                unfold Cop.sem_cmp; rewrite Heq; unfold Cop.cmp_ptr; ss; des_ifs_safe; 
-                  unfold Mem.weak_valid_pointer in *; clarify.
-        * eapply step_weak_valid_pointer; et. i. sim_red. eapply step_weak_valid_pointer; et. i.
-          des_ifs; sim_red; eapplyf NEXT; i; ss; clarify;
-          unfold Cop.sem_cmp; rewrite Heq; unfold Cop.cmp_ptr; ss; des_ifs_safe; unfold Mem.weak_valid_pointer in *; clarify;
-          unfold Val.of_bool; des_ifs. 
-        * unfold ccallU. sim_red. ss. repeat (sim_tau; sim_red). unfold valid_pointerF. sim_red.
-          repeat (sim_tau; sim_red). rewrite PSTATE. sim_red. repeat (sim_tau; sim_red).
-          unfold valid_pointerF. sim_red.
-          repeat (sim_tau; sim_red). rewrite PSTATE. sim_red. repeat (sim_tau; sim_red).
-          repeat match goal with | |- context [Mem.perm_dec ?x ?y ?z ?w ?a] => destruct (Mem.perm_dec x y z w a) end; sim_red;
-            eapplyf NEXT; i; ss; clarify;
-              unfold Cop.sem_cmp; rewrite Heq; unfold Cop.cmp_ptr; ss; unfold Mem.valid_pointer in *;
-                destruct (eq_block _); des_ifs_safe;
-          try solve [eapply map_blk_inj in e0; et; try contradiction];
-          repeat (destruct (Mem.perm_dec _)); inv MM; unfold Mem.perm in *; ss.
-      + unfold cmplu_bool_c; des_ifs; try sim_red;
-          try solve [eapplyf NEXT; i; ss; clarify; unfold Cop.sem_cmp; rewrite Heq; unfold Cop.cmp_ptr; des_ifs_safe].
-          1: eapplyf NEXT; i; ss; clarify; unfold Cop.sem_cmp; rewrite Heq; unfold Cop.cmp_ptr; des_ifs_safe.
-          2: eapply step_weak_valid_pointer; et; i; des_ifs; sim_red; eapplyf NEXT; i; ss; clarify;
-                unfold Cop.sem_cmp; rewrite Heq; unfold Cop.cmp_ptr; ss; des_ifs_safe; 
-                  unfold Mem.weak_valid_pointer in *; clarify.
-          all: unfold Val.of_bool; unfold Val.cmplu_bool; des_ifs; unfold Int64.cmpu; rewrite Heq1; ss.
-      + unfold cmplu_bool_c; des_ifs; try sim_red;
-          try solve [eapplyf NEXT; i; ss; clarify; unfold Cop.sem_cmp; rewrite Heq; unfold Cop.cmp_ptr; des_ifs_safe].
-        * eapply step_weak_valid_pointer; et; i; des_ifs; sim_red; eapplyf NEXT; i; ss; clarify;
-                unfold Cop.sem_cmp; rewrite Heq; unfold Cop.cmp_ptr; ss; des_ifs_safe; 
-                  unfold Mem.weak_valid_pointer in *; clarify.
-        * eapply step_weak_valid_pointer; et. i. sim_red. eapply step_weak_valid_pointer; et. i.
-          des_ifs; sim_red; eapplyf NEXT; i; ss; clarify;
-          unfold Cop.sem_cmp; rewrite Heq; unfold Cop.cmp_ptr; ss; des_ifs_safe; unfold Mem.weak_valid_pointer in *; clarify;
-          unfold Val.of_bool; des_ifs. 
-        * unfold ccallU. sim_red. ss. repeat (sim_tau; sim_red). unfold valid_pointerF. sim_red.
-          repeat (sim_tau; sim_red). rewrite PSTATE. sim_red. repeat (sim_tau; sim_red).
-          unfold valid_pointerF. sim_red.
-          repeat (sim_tau; sim_red). rewrite PSTATE. sim_red. repeat (sim_tau; sim_red).
-          repeat match goal with | |- context [Mem.perm_dec ?x ?y ?z ?w ?a] => destruct (Mem.perm_dec x y z w a) end; sim_red;
-            eapplyf NEXT; i; ss; clarify;
-              unfold Cop.sem_cmp; rewrite Heq; unfold Cop.cmp_ptr; ss; unfold Mem.valid_pointer in *;
-                destruct (eq_block _); des_ifs_safe;
-          try solve [eapply map_blk_inj in e0; et; try contradiction];
-          repeat (destruct (Mem.perm_dec _)); inv MM; unfold Mem.perm in *; ss.
-    + unfold sem_binarith_c. sim_red. eapply step_sem_cast; et. i. destruct optv; sim_red;
-        try solve [ eapplyf NEXT; i; clarify; unfold Cop.sem_binary_operation, Cop.sem_cmp; unfold Cop.sem_binarith; rewrite Heq;
-                  try (erewrite H by et); try (erewrite H0 by et); try (erewrite H1 by et); try (erewrite H2 by et); ss].
-      eapply step_sem_cast; et. i. destruct optv; try sim_red;
-        try solve [eapplyf NEXT; i; clarify; unfold Cop.sem_binary_operation, Cop.sem_cmp; unfold Cop.sem_binarith; rewrite Heq;
-                  try (erewrite H by et); try (erewrite H0 by et); try (erewrite H1 by et); try (erewrite H2 by et); ss].
-      des_ifs; sim_red; 
-        eapplyf NEXT; i; clarify; unfold Cop.sem_binary_operation, Cop.sem_cmp; unfold Cop.sem_binarith; 
-          rewrite Heq in *; rewrite Heq0 in *;
-            try (erewrite H by et); try (erewrite H0 by et); try (erewrite H1 by et); try (erewrite H2 by et); ss.
-      all: unfold Val.of_bool; unfold Val.cmplu_bool; des_ifs; unfold Int64.cmpu; rewrite Heq1; ss.
+    - destruct Cop.classify_cmp eqn:?; remove_UBcase.
+      + eapply step_cmp_ptr; et. i. sim_red. eapply NEXT. ss. unfold Cop.sem_cmp. des_ifs.
+        rewrite H. unfold Val.of_bool. des_ifs.
+      + eapply step_cmp_ptr; et. i. sim_red. eapply NEXT. ss. unfold Cop.sem_cmp. des_ifs.
+        unfold Vptrofs in *. des_ifs. ss.
+        rewrite H. unfold Val.of_bool. des_ifs.
+      + eapply step_cmp_ptr; et. i. sim_red. eapply NEXT. ss. unfold Cop.sem_cmp. des_ifs.
+        unfold Vptrofs in *. des_ifs. ss.
+        rewrite H. unfold Val.of_bool. des_ifs.
+      + eapply step_cmp_ptr; et. i. sim_red. eapply NEXT. ss. unfold Cop.sem_cmp. des_ifs.
+        unfold Vptrofs in *. des_ifs. ss.
+        rewrite H. unfold Val.of_bool. des_ifs.
+      + eapply step_cmp_ptr; et. i. sim_red. eapply NEXT. ss. unfold Cop.sem_cmp. des_ifs.
+        rewrite H. unfold Val.of_bool. des_ifs.
+      + eapply step_cmp_ptr; et. i. sim_red. eapply NEXT. ss. unfold Cop.sem_cmp. des_ifs.
+        unfold Vptrofs in *. des_ifs. ss.
+        rewrite H. unfold Val.of_bool. des_ifs.
+      + eapply step_cmp_ptr; et. i. sim_red. eapply NEXT. simpl. unfold Cop.sem_cmp. des_ifs.
+        simpl map_val in H.
+        rewrite H. unfold Val.of_bool. des_ifs.
+      + unfold sem_binarith_c. sim_red. eapply step_sem_cast; et. i. sim_red.
+        eapply step_sem_cast; et. i. remove_UBcase.
+        all: apply NEXT; unfold Cop.sem_binary_operation, Cop.sem_cmp, Cop.sem_binarith; rewrite Heq; des_ifs.
+        all: unfold Val.of_bool; des_ifs; ss; clarify.
+    - destruct Cop.classify_cmp eqn:?; remove_UBcase.
+      + eapply step_cmp_ptr; et. i. sim_red. eapply NEXT. ss. unfold Cop.sem_cmp. des_ifs.
+        rewrite H. unfold Val.of_bool. des_ifs.
+      + eapply step_cmp_ptr; et. i. sim_red. eapply NEXT. ss. unfold Cop.sem_cmp. des_ifs.
+        unfold Vptrofs in *. des_ifs. ss.
+        rewrite H. unfold Val.of_bool. des_ifs.
+      + eapply step_cmp_ptr; et. i. sim_red. eapply NEXT. ss. unfold Cop.sem_cmp. des_ifs.
+        unfold Vptrofs in *. des_ifs. ss.
+        rewrite H. unfold Val.of_bool. des_ifs.
+      + eapply step_cmp_ptr; et. i. sim_red. eapply NEXT. ss. unfold Cop.sem_cmp. des_ifs.
+        unfold Vptrofs in *. des_ifs. ss.
+        rewrite H. unfold Val.of_bool. des_ifs.
+      + eapply step_cmp_ptr; et. i. sim_red. eapply NEXT. ss. unfold Cop.sem_cmp. des_ifs.
+        rewrite H. unfold Val.of_bool. des_ifs.
+      + eapply step_cmp_ptr; et. i. sim_red. eapply NEXT. ss. unfold Cop.sem_cmp. des_ifs.
+        unfold Vptrofs in *. des_ifs. ss.
+        rewrite H. unfold Val.of_bool. des_ifs.
+      + eapply step_cmp_ptr; et. i. sim_red. eapply NEXT. simpl. unfold Cop.sem_cmp. des_ifs.
+        simpl map_val in H.
+        rewrite H. unfold Val.of_bool. des_ifs.
+      + unfold sem_binarith_c. sim_red. eapply step_sem_cast; et. i. sim_red.
+        eapply step_sem_cast; et. i. remove_UBcase.
+        all: apply NEXT; unfold Cop.sem_binary_operation, Cop.sem_cmp, Cop.sem_binarith; rewrite Heq; des_ifs.
+        all: unfold Val.of_bool; des_ifs; ss; clarify.
+    - destruct Cop.classify_cmp eqn:?; remove_UBcase.
+      + eapply step_cmp_ptr; et. i. sim_red. eapply NEXT. ss. unfold Cop.sem_cmp. des_ifs.
+        rewrite H. unfold Val.of_bool. des_ifs.
+      + eapply step_cmp_ptr; et. i. sim_red. eapply NEXT. ss. unfold Cop.sem_cmp. des_ifs.
+        unfold Vptrofs in *. des_ifs. ss.
+        rewrite H. unfold Val.of_bool. des_ifs.
+      + eapply step_cmp_ptr; et. i. sim_red. eapply NEXT. ss. unfold Cop.sem_cmp. des_ifs.
+        unfold Vptrofs in *. des_ifs. ss.
+        rewrite H. unfold Val.of_bool. des_ifs.
+      + eapply step_cmp_ptr; et. i. sim_red. eapply NEXT. ss. unfold Cop.sem_cmp. des_ifs.
+        unfold Vptrofs in *. des_ifs. ss.
+        rewrite H. unfold Val.of_bool. des_ifs.
+      + eapply step_cmp_ptr; et. i. sim_red. eapply NEXT. ss. unfold Cop.sem_cmp. des_ifs.
+        rewrite H. unfold Val.of_bool. des_ifs.
+      + eapply step_cmp_ptr; et. i. sim_red. eapply NEXT. ss. unfold Cop.sem_cmp. des_ifs.
+        unfold Vptrofs in *. des_ifs. ss.
+        rewrite H. unfold Val.of_bool. des_ifs.
+      + eapply step_cmp_ptr; et. i. sim_red. eapply NEXT. simpl. unfold Cop.sem_cmp. des_ifs.
+        simpl map_val in H.
+        rewrite H. unfold Val.of_bool. des_ifs.
+      + unfold sem_binarith_c. sim_red. eapply step_sem_cast; et. i. sim_red.
+        eapply step_sem_cast; et. i. remove_UBcase.
+        all: apply NEXT; unfold Cop.sem_binary_operation, Cop.sem_cmp, Cop.sem_binarith; rewrite Heq; des_ifs.
+        all: unfold Val.of_bool; des_ifs; ss; clarify.
+    - destruct Cop.classify_cmp eqn:?; remove_UBcase.
+      + eapply step_cmp_ptr; et. i. sim_red. eapply NEXT. ss. unfold Cop.sem_cmp. des_ifs.
+        rewrite H. unfold Val.of_bool. des_ifs.
+      + eapply step_cmp_ptr; et. i. sim_red. eapply NEXT. ss. unfold Cop.sem_cmp. des_ifs.
+        unfold Vptrofs in *. des_ifs. ss.
+        rewrite H. unfold Val.of_bool. des_ifs.
+      + eapply step_cmp_ptr; et. i. sim_red. eapply NEXT. ss. unfold Cop.sem_cmp. des_ifs.
+        unfold Vptrofs in *. des_ifs. ss.
+        rewrite H. unfold Val.of_bool. des_ifs.
+      + eapply step_cmp_ptr; et. i. sim_red. eapply NEXT. ss. unfold Cop.sem_cmp. des_ifs.
+        unfold Vptrofs in *. des_ifs. ss.
+        rewrite H. unfold Val.of_bool. des_ifs.
+      + eapply step_cmp_ptr; et. i. sim_red. eapply NEXT. ss. unfold Cop.sem_cmp. des_ifs.
+        rewrite H. unfold Val.of_bool. des_ifs.
+      + eapply step_cmp_ptr; et. i. sim_red. eapply NEXT. ss. unfold Cop.sem_cmp. des_ifs.
+        unfold Vptrofs in *. des_ifs. ss.
+        rewrite H. unfold Val.of_bool. des_ifs.
+      + eapply step_cmp_ptr; et. i. sim_red. eapply NEXT. simpl. unfold Cop.sem_cmp. des_ifs.
+        simpl map_val in H.
+        rewrite H. unfold Val.of_bool. des_ifs.
+      + unfold sem_binarith_c. sim_red. eapply step_sem_cast; et. i. sim_red.
+        eapply step_sem_cast; et. i. remove_UBcase.
+        all: apply NEXT; unfold Cop.sem_binary_operation, Cop.sem_cmp, Cop.sem_binarith; rewrite Heq; des_ifs.
+        all: unfold Val.of_bool; des_ifs; ss; clarify.
+    - destruct Cop.classify_cmp eqn:?; remove_UBcase.
+      + eapply step_cmp_ptr; et. i. sim_red. eapply NEXT. ss. unfold Cop.sem_cmp. des_ifs.
+        rewrite H. unfold Val.of_bool. des_ifs.
+      + eapply step_cmp_ptr; et. i. sim_red. eapply NEXT. ss. unfold Cop.sem_cmp. des_ifs.
+        unfold Vptrofs in *. des_ifs. ss.
+        rewrite H. unfold Val.of_bool. des_ifs.
+      + eapply step_cmp_ptr; et. i. sim_red. eapply NEXT. ss. unfold Cop.sem_cmp. des_ifs.
+        unfold Vptrofs in *. des_ifs. ss.
+        rewrite H. unfold Val.of_bool. des_ifs.
+      + eapply step_cmp_ptr; et. i. sim_red. eapply NEXT. ss. unfold Cop.sem_cmp. des_ifs.
+        unfold Vptrofs in *. des_ifs. ss.
+        rewrite H. unfold Val.of_bool. des_ifs.
+      + eapply step_cmp_ptr; et. i. sim_red. eapply NEXT. ss. unfold Cop.sem_cmp. des_ifs.
+        rewrite H. unfold Val.of_bool. des_ifs.
+      + eapply step_cmp_ptr; et. i. sim_red. eapply NEXT. ss. unfold Cop.sem_cmp. des_ifs.
+        unfold Vptrofs in *. des_ifs. ss.
+        rewrite H. unfold Val.of_bool. des_ifs.
+      + eapply step_cmp_ptr; et. i. sim_red. eapply NEXT. simpl. unfold Cop.sem_cmp. des_ifs.
+        simpl map_val in H.
+        rewrite H. unfold Val.of_bool. des_ifs.
+      + unfold sem_binarith_c. sim_red. eapply step_sem_cast; et. i. sim_red.
+        eapply step_sem_cast; et. i. remove_UBcase.
+        all: apply NEXT; unfold Cop.sem_binary_operation, Cop.sem_cmp, Cop.sem_binarith; rewrite Heq; des_ifs.
+        all: unfold Val.of_bool; des_ifs; ss; clarify.
+    - destruct Cop.classify_cmp eqn:?; remove_UBcase.
+      + eapply step_cmp_ptr; et. i. sim_red. eapply NEXT. ss. unfold Cop.sem_cmp. des_ifs.
+        rewrite H. unfold Val.of_bool. des_ifs.
+      + eapply step_cmp_ptr; et. i. sim_red. eapply NEXT. ss. unfold Cop.sem_cmp. des_ifs.
+        unfold Vptrofs in *. des_ifs. ss.
+        rewrite H. unfold Val.of_bool. des_ifs.
+      + eapply step_cmp_ptr; et. i. sim_red. eapply NEXT. ss. unfold Cop.sem_cmp. des_ifs.
+        unfold Vptrofs in *. des_ifs. ss.
+        rewrite H. unfold Val.of_bool. des_ifs.
+      + eapply step_cmp_ptr; et. i. sim_red. eapply NEXT. ss. unfold Cop.sem_cmp. des_ifs.
+        unfold Vptrofs in *. des_ifs. ss.
+        rewrite H. unfold Val.of_bool. des_ifs.
+      + eapply step_cmp_ptr; et. i. sim_red. eapply NEXT. ss. unfold Cop.sem_cmp. des_ifs.
+        rewrite H. unfold Val.of_bool. des_ifs.
+      + eapply step_cmp_ptr; et. i. sim_red. eapply NEXT. ss. unfold Cop.sem_cmp. des_ifs.
+        unfold Vptrofs in *. des_ifs. ss.
+        rewrite H. unfold Val.of_bool. des_ifs.
+      + eapply step_cmp_ptr; et. i. sim_red. eapply NEXT. simpl. unfold Cop.sem_cmp. des_ifs.
+        simpl map_val in H.
+        rewrite H. unfold Val.of_bool. des_ifs.
+      + unfold sem_binarith_c. sim_red. eapply step_sem_cast; et. i. sim_red.
+        eapply step_sem_cast; et. i. remove_UBcase.
+        all: apply NEXT; unfold Cop.sem_binary_operation, Cop.sem_cmp, Cop.sem_binarith; rewrite Heq; des_ifs.
+        all: unfold Val.of_bool; des_ifs; ss; clarify.
   Qed.
 
-  Lemma _step_eval pstate ge ce f_table modl cprog sk tge le tle e te m tm
+  Lemma _step_eval pstate ge ce tce f_table modl cprog sk tge le tle e te m tm
     (PSTATE: pstate "Mem"%string = m↑)
-    (EQ1: ce = ge.(genv_cenv)) 
+    (EQ1: tce = ge.(genv_cenv)) 
     (EQ2: tge = ge.(genv_genv))
     (EQ3: f_table = (ModL.add Mem modl).(ModL.enclose))
     (MGE: match_ge sk tge)
     (ME: match_e sk tge e te)
     (MLE: match_le sk tge le tle)
+    (MCE: match_ce ce tce)
     (MM: match_mem sk tge m tm)
  r b tcode tf tcont mn a
  :
   (forall ktr1,
-    (forall blk ofs bf, 
-      eval_lvalue ge te tle tm a (map_blk sk tge blk) ofs bf ->
+    (forall vp, 
+      eval_lvalue ge te tle tm a (map_val sk tge vp) ->
       paco4
         (_sim (ModL.compile (ModL.add Mem modl)) (semantics2 cprog)) r true b
-        (ktr1 (pstate, (blk, (ofs, bf))))
+        (ktr1 (pstate, vp))
         (State tf tcode tcont te tle tm)) 
     ->
     paco4
       (_sim (ModL.compile (ModL.add Mem modl)) (semantics2 cprog)) r true b
-      (`r0: (p_state * (Values.block * (ptrofs * bitfield))) <- 
+      (`r0: (p_state * val) <- 
         (EventsL.interp_Es
           (prog f_table)
           (transl_all mn (eval_lvalue_c sk ce e le a)) 
@@ -1286,8 +1303,6 @@ Section PROOF.
   Proof.
     induction a.
     1,2,3,4 : split; i; remove_UBcase; eapply H; try econs.
-    9,10 : des; split; i; remove_UBcase; ss; unfold Vptrofs; 
-          eapply H; et; des_ifs_safe; econs.
     2,4,5,6,7 : des; split; i; remove_UBcase; ss.
     - split; i; ss.
       + remove_UBcase; eapply H; et. 
@@ -1297,43 +1312,77 @@ Section PROOF.
         * econs. hexploit env_match_some; et.
         * econs 2; try solve [eapply env_match_none; et]. inv MGE. eapply MGE0; et.
     - unfold unwrapU. remove_UBcase. eapply H; et. econs. inv MLE. eapply ML. et.
-    - eapply IHa. i. subst. destruct bf; try sim_red; try sim_triggerUB. eapply H; et. econs; et.
-    - eapply IHa0. i. sim_red. eapply step_unary_op; et. i. sim_red.
-      destruct optv; try sim_triggerUB. sim_red. eapply H; et. econs; et.
-    - eapply IHa3. i. sim_red. eapply IHa0. i. sim_red. eapply step_binary_op; et.
-      i. sim_red. destruct optv; try sim_triggerUB. sim_red. eapply H; et. econs; et.
-    - eapply IHa0. i. sim_red. eapply step_sem_cast; et. i.
-      sim_red. unfold unwrapU. remove_UBcase. eapply H; et. econs; et. 
+    - eapply IHa. i. eapply H; et. econs; et.
+    - eapply IHa0. i. eapply step_unary_op; et. i. eapply H; et. econs; et.
+    - eapply IHa3. i. sim_red. eapply IHa0. i. eapply step_binary_op; et.
+      i. eapply H; et. econs; et.
+    - eapply IHa0. i. eapply step_sem_cast; et. i. eapply H; et. econs; et. 
     - des; split; i; ss; remove_UBcase; eapply IHa0; i; remove_UBcase.
-      + eapply H. econs; et.
-      + eapply step_deref_loc; et. i. sim_red. eapply H. econs; et. econs;et.
+      + eapply H. econs; et. destruct v; ss.
+      + eapply step_deref_loc; et. i. sim_red. eapply H. econs; et. econs;et. destruct v; ss.
     - des. split; i; ss; sim_red; eapply IHa0; i; subst. 
-      + remove_UBcase; unfold unwrapU; remove_UBcase; remove_UBcase; eapply H; et; [econs|econs 5]; et.
-      + remove_UBcase; unfold unwrapU; remove_UBcase; remove_UBcase; 
-        eapply step_deref_loc; et; i; sim_red; eapply H; et; econs; et; [econs|econs 5]; et.
+      + remove_UBcase; unfold unwrapU; remove_UBcase; remove_UBcase; eapply H; et.
+        * econs; et. { destruct v; ss. }
+          { inv MCE. rewrite <- MCE0 in Heq2. apply Maps.PTree.elements_complete. et. }
+          2:{ des_ifs. destruct v; ss. }
+          { unfold ClightPlusExprgen.field_offset in Heq3.
+            clear - Heq3 MCE. unfold field_offset. set 0%Z as d in *.
+            clearbody d. destruct c. ss. revert i d Heq3.
+            induction co_members; ss. i. des_ifs.
+            { erewrite match_alignof; et. } apply IHco_members.
+            erewrite match_alignof; et. erewrite match_sizeof; et. }
+        * econs 5; et. { destruct v; ss. }
+          inv MCE. rewrite <- MCE0 in Heq1. apply Maps.PTree.elements_complete. et.
+      + remove_UBcase; unfold unwrapU; remove_UBcase; remove_UBcase;
+        eapply step_deref_loc; et; i; sim_red; eapply H; et; econs; et.
+        * econs; et. { destruct v; ss. }
+          { inv MCE. rewrite <- MCE0 in Heq2. apply Maps.PTree.elements_complete. et. }
+          2:{ des_ifs. destruct v; ss. }
+          { unfold ClightPlusExprgen.field_offset in Heq3.
+            clear - Heq3 MCE. unfold field_offset. set 0%Z as d in *.
+            clearbody d. destruct c. ss. revert i d Heq3.
+            induction co_members; ss. i. des_ifs.
+            { erewrite match_alignof; et. } apply IHco_members.
+            erewrite match_alignof; et. erewrite match_sizeof; et. }
+        * econs 5; et. { destruct v; ss. }
+          inv MCE. rewrite <- MCE0 in Heq1. apply Maps.PTree.elements_complete. et.
+    - split; i.
+      + ss. remove_UBcase.
+      + ss. sim_red. apply H.
+        replace (map_val sk _ _) with (Vptrofs (Ptrofs.repr (ClightPlusExprgen.sizeof ce t0))).
+        2:{ unfold Vptrofs. des_ifs. }
+        erewrite <- match_sizeof; et.
+        replace tce with (ge.(genv_cenv)). econs.
+    - split; i.
+      + ss. remove_UBcase.
+      + ss. sim_red. apply H.
+        replace (map_val sk _ _) with (Vptrofs (Ptrofs.repr (ClightPlusExprgen.alignof ce t0))).
+        2:{ unfold Vptrofs. des_ifs. }
+        erewrite <- match_alignof; et.
+        replace tce with (ge.(genv_cenv)). econs.
   Qed.
-    
 
-  Lemma step_eval_lvalue pstate ge ce f_table modl cprog sk tge le tle e te m tm
+  Lemma step_eval_lvalue pstate ge tce ce f_table modl cprog sk tge le tle e te m tm
     (PSTATE: pstate "Mem"%string = m↑)
-    (EQ1: ce = ge.(genv_cenv)) 
+    (EQ1: tce = ge.(genv_cenv)) 
     (EQ2: tge = ge.(genv_genv)) 
     (EQ3: f_table = (ModL.add Mem modl).(ModL.enclose))
     (MGE: match_ge sk tge)
     (ME: match_e sk tge e te)
     (MLE: match_le sk tge le tle)
+    (MCE: match_ce ce tce)
     (MM: match_mem sk tge m tm)
  r b tcode tf tcont mn a ktr
-    (NEXT: forall blk ofs bf, 
-            eval_lvalue ge te tle tm a (map_blk sk tge blk) ofs bf ->
+    (NEXT: forall vp, 
+            eval_lvalue ge te tle tm a (map_val sk tge vp) ->
             paco4
               (_sim (ModL.compile (ModL.add Mem modl)) (semantics2 cprog)) r true b
-              (ktr (pstate, (blk, (ofs, bf))))
+              (ktr (pstate, vp))
               (State tf tcode tcont te tle tm))
   :
     paco4
       (_sim (ModL.compile (ModL.add Mem modl)) (semantics2 cprog)) r true b
-      (`r0: (p_state * (Values.block * (ptrofs * bitfield))) <- 
+      (`r0: (p_state * val) <- 
         (EventsL.interp_Es
           (prog f_table)
           (transl_all mn (eval_lvalue_c sk ce e le a)) 
@@ -1341,14 +1390,15 @@ Section PROOF.
       (State tf tcode tcont te tle tm).
   Proof. hexploit _step_eval; et. i. des. et. Qed.
 
-  Lemma step_eval_expr pstate ge ce f_table modl cprog sk tge le tle e te m tm
+  Lemma step_eval_expr pstate ge tce ce f_table modl cprog sk tge le tle e te m tm
     (PSTATE: pstate "Mem"%string = m↑)
-    (EQ1: ce = ge.(genv_cenv)) 
+    (EQ1: tce = ge.(genv_cenv)) 
     (EQ2: tge = ge.(genv_genv)) 
     (EQ3: f_table = (ModL.add Mem modl).(ModL.enclose))
     (MGE: match_ge sk tge)
     (ME: match_e sk tge e te)
     (MLE: match_le sk tge le tle)
+    (MCE: match_ce ce tce)
     (MM: match_mem sk tge m tm)
  r b tcode tf tcont mn a ktr
     (NEXT: forall v v', 
@@ -1367,7 +1417,6 @@ Section PROOF.
           (transl_all mn (eval_expr_c sk ce e le a))
           pstate);; ktr r0)
       (State tf tcode tcont te tle tm). 
-  Proof. hexploit _step_eval; et. i. des. et. Qed. *)
-          
+  Proof. hexploit _step_eval; et. i. des. et. Qed.
 
 End PROOF.
